restore map group definitions (with some admits left)

src/cddl/spec/CDDL.Spec.MapGroup.Base.fst
@@ -1,32 +1,51 @@
-module CDDL.Spec.MapGroupGen.Base
+module CDDL.Spec.MapGroup.Base
+open CBOR.Spec.API.Type
 
 module FE = FStar.FunctionalExtensionality
+module MPS = CBOR.Spec.API.MapPairSet
 
-let cbor_map = ghost_map Cbor.raw_data_item Cbor.raw_data_item
-
-let map_group_item : Type0 =
+let map_group_item : eqtype =
   (cbor_map & cbor_map)
 
-noeq
+let mps_for_all
+  (f: (map_group_item -> bool))
+  (m: MPS.t)
+: Pure bool
+    (requires True)
+    (ensures fun b -> b <==> (forall k . MPS.mem k m ==> f k))
+= let b = MPS.filter f m = m in // HERE we use the fact that the map pair set is eqtype
+  assert (b == true <==> MPS.equal (MPS.filter f m) m);
+  b
+
 type map_group_sem_result =
-| MapGroupResult of FStar.GSet.set map_group_item
+| MapGroupResult of MPS.t
 | MapGroupCutFailure
 
-let map_group_post'
+let map_group_post'_prop
   (l: cbor_map)
-  (res: FStar.GSet.set map_group_item)
+  (res: MPS.t)
 : Tot prop
 =
       forall l' .
-      FStar.GSet.mem l' res ==>  map_group_item_post l l'
+      MPS.mem l' res ==>  map_group_item_post l l'
+
+let map_group_post'_t (l: cbor_map) : Tot eqtype = (res: MPS.t { map_group_post'_prop l res })
+
+let map_group_post'
+  (l: cbor_map)
+  (res: MPS.t)
+: Pure bool
+    (requires True)
+    (ensures fun b -> b <==> map_group_post'_prop l res)
+= mps_for_all (map_group_item_post l) res
 
 let map_group_post
   (l: cbor_map)
   (res: map_group_sem_result)
-: Tot prop
+: Tot bool
 = match res with
   | MapGroupResult res -> map_group_post' l res
-  | MapGroupCutFailure -> True
+  | MapGroupCutFailure -> true
 
 let map_group_codom
   (l: cbor_map)
@@ -36,37 +55,52 @@ let map_group_codom
   })
 
 let map_group : Type0 =
-  FE.restricted_g_t
+  FE.restricted_t
     (cbor_map)
     (map_group_codom)
 
 let map_group_always_false : map_group =
-  FE.on_dom_g cbor_map #map_group_codom
-    (fun _ -> MapGroupResult FStar.GSet.empty)
+  FE.on_dom cbor_map #map_group_codom
+    (fun _ -> MapGroupResult MPS.empty)
 
 let map_group_nop : map_group =
-  FE.on_dom_g cbor_map #map_group_codom
-    (fun l -> MapGroupResult (FStar.GSet.singleton (ghost_map_empty, l)))
-
-let ghost_map_is_empty
-  (#key #value: Type)
-  (m: ghost_map key value)
-: Ghost bool
-  (requires True)
-  (ensures fun res -> res == true <==> m == ghost_map_empty)
-= FStar.StrongExcludedMiddle.strong_excluded_middle (m == ghost_map_empty)
+  FE.on_dom cbor_map #map_group_codom
+    (fun l -> MapGroupResult (MPS.singleton (cbor_map_empty, l)))
 
 let map_group_end : map_group =
-  FE.on_dom_g cbor_map #map_group_codom
-    (fun l -> if ghost_map_is_empty l then map_group_nop l else map_group_always_false l)
+  FE.on_dom cbor_map #map_group_codom
+    (fun l -> if l = cbor_map_empty then map_group_nop l else map_group_always_false l)
+
+let cbor_map_singleton_inj
+  (k1 v1 k2 v2: cbor)
+: Lemma
+  (requires (cbor_map_singleton k1 v1 == cbor_map_singleton k2 v2))
+  (ensures (k1 == k2 /\ v1 == v2))
+  [SMTPat (cbor_map_singleton k1 v1); SMTPat (cbor_map_singleton k2 v2)]
+= assert (forall x . cbor_map_mem x (cbor_map_singleton k1 v1) ==> x == (k1, v1));
+  assert (forall x . cbor_map_mem x (cbor_map_singleton k2 v2) ==> x == (k2, v2))
 
 unfold
-let map_group_match_item_witness_pred (key value: typ) (l: cbor_map) (l': cbor_map & cbor_map) (x: Cbor.raw_data_item & Cbor.raw_data_item) : Tot prop =
+let map_group_match_item_witness_pred (key value: typ) (l: cbor_map) (l': cbor_map & cbor_map) (x: cbor & cbor) : Tot prop =
   map_group_item_post l l' /\
-  fst l' == ghost_map_singleton (fst x) (snd x) /\
+  fst l' == cbor_map_singleton (fst x) (snd x) /\
   key (fst x) /\
   value (snd x)
 
+let map_group_match_item_witness_pred_inj (key value: typ) (l: cbor_map) (l': cbor_map & cbor_map) (x1 x2: (cbor & cbor)) : Lemma
+  (requires (map_group_match_item_witness_pred key value l l' x1 /\ map_group_match_item_witness_pred key value l l' x2))
+  (ensures (x1 == x2))
+= ()
+
+let map_group_match_item_witness_bool (key value: typ) (l: cbor_map) (l': cbor_map & cbor_map) (x: cbor & cbor) : Pure bool
+  (requires True)
+  (ensures fun b -> b <==> map_group_match_item_witness_pred key value l l' x)
+= map_group_item_post l l' &&
+  fst l' = cbor_map_singleton (fst x) (snd x) &&
+  key (fst x) &&
+  value (snd x)
+
+(*
 let pred2_equiv_trans
   (#t #t': Type)
   (p1 p2 p3: t -> t' -> prop)
@@ -79,87 +113,280 @@ let pred2_equiv_trans
     (forall x x' . p1 x x' <==> p3 x x')
   ))
 = ()
+*)
 
-let map_group_match_item_comprehend
+let mps_union_assoc
+  (x1 x2 x3: MPS.t)
+: Lemma
+  (ensures (MPS.union (MPS.union x1 x2) x3 == MPS.union x1 (MPS.union x2 x3)))
+  [SMTPatOr [
+    [SMTPat (MPS.union (MPS.union x1 x2) x3)];
+    [SMTPat (MPS.union x1 (MPS.union x2 x3))];
+  ]]
+= assert (MPS.equal (MPS.union (MPS.union x1 x2) x3) (MPS.union x1 (MPS.union x2 x3)))
+
+let mps_union_comm
+  (x1 x2: MPS.t)
+: Lemma
+  (ensures (MPS.union x1 x2 == MPS.union x2 x1))
+  [SMTPat (MPS.union x1 x2)]
+= assert (MPS.equal (MPS.union x1 x2) (MPS.union x2 x1))
+
+let map_group_match_item_op
   (key value: typ)
   (l: cbor_map)
-  l'
-: GTot bool
-=
-    FStar.StrongExcludedMiddle.strong_excluded_middle (exists x .
-      map_group_match_item_witness_pred key value l l' x
-    )
+  (accu: map_group_post'_t l)
+  (k: cbor)
+: Tot (map_group_post'_t l)
+= match cbor_map_get l k with
+  | None -> accu
+  | Some v ->
+    if key k && value v
+    then
+      let l1 = cbor_map_singleton k v in
+      let l2 = cbor_map_sub l l1 in
+      MPS.union accu (MPS.singleton (l1, l2))
+    else accu
 
-let map_group_match_item' (key value: typ) (l: cbor_map) : FStar.GSet.set map_group_item =
-  FStar.GSet.comprehend (map_group_match_item_comprehend key value l)
+let map_group_match_item_op_implies
+  (key value: typ)
+  (l: cbor_map)
+  (accu: map_group_post'_t l)
+  (k: cbor)
+  (l': map_group_item)
+: Lemma
+  (requires (
+    MPS.mem l' (map_group_match_item_op key value l accu k)
+  ))
+  (ensures (MPS.mem l' accu \/ exists x . map_group_match_item_witness_pred key value l l' (k, x)))
+= ()
 
-let map_group_match_item_elim (key value: typ) (l: cbor_map) l' : Ghost _
-  (requires (FStar.GSet.mem l' (map_group_match_item' key value l)))
+let map_group_match_item_op_implies_recip
+  (key value: typ)
+  (l: cbor_map)
+  (accu: map_group_post'_t l)
+  (k: cbor)
+  (l': map_group_item)
+  (x: cbor)
+: Lemma
+  (requires (
+    map_group_match_item_witness_pred key value l l' (k, x)
+  ))
+  (ensures (MPS.mem l' (map_group_match_item_op key value l accu k)))
+= assert (cbor_map_defined k l);
+  let Some v = cbor_map_get l k in
+  assert (x == v);
+  assert (key k);
+  assert (value v);
+  assert (cbor_map_equal (fst l') (cbor_map_singleton k v));
+  assert (cbor_map_equal (snd l') (cbor_map_sub l (fst l')))
+
+let map_group_match_item_op_eq
+  (key value: typ)
+  (l: cbor_map)
+  (accu: map_group_post'_t l)
+  (k: cbor)
+  (l': map_group_item)
+: Lemma
+  (ensures (MPS.mem l' (map_group_match_item_op key value l accu k) <==> (MPS.mem l' accu \/ exists x . map_group_match_item_witness_pred key value l l' x /\ fst x == k)))
+  [SMTPat (MPS.mem l' (map_group_match_item_op key value l accu k))]
+= Classical.forall_intro (Classical.move_requires (map_group_match_item_op_implies_recip key value l accu k l'))
+
+let rec list_fold_map_group_match_item_op_eq
+  (key value: typ)
+  (l: cbor_map)
+  (accu: map_group_post'_t l)
+  (ls: list cbor)
+  (l': map_group_item)
+: Lemma
+  (ensures (MPS.mem l' (List.Tot.fold_left (map_group_match_item_op key value l) accu ls) <==> (MPS.mem l' accu \/ exists x . map_group_match_item_witness_pred key value l l' x /\ List.Tot.memP (fst x) ls)))
+  (decreases ls)
+  [SMTPat (MPS.mem l' (List.Tot.fold_left (map_group_match_item_op key value l) accu ls))]
+= match ls with
+  | [] -> ()
+  | a :: q -> list_fold_map_group_match_item_op_eq key value l (map_group_match_item_op key value l accu a) q l'
+
+let map_group_match_item' (key value: typ) (l: cbor_map) : map_group_post'_t l =
+  cbor_map_fold (map_group_match_item_op key value l) MPS.empty l
+
+let map_group_match_item'_eq (key value: typ) (l: cbor_map) (l': map_group_item) : Lemma
+  (ensures (MPS.mem l' (map_group_match_item' key value l) <==> exists x . map_group_match_item_witness_pred key value l l' x))
+  [SMTPat (MPS.mem l' (map_group_match_item' key value l))]
+= cbor_map_fold_eq (map_group_match_item_op key value l) MPS.empty l (cbor_map_key_list l)
+
+let mps_singleton_elim
+  (s: MPS.t)
+: Pure map_group_item
+    (requires MPS.cardinality s == 1)
+    (ensures fun x -> MPS.equal s (MPS.singleton x))
+= let l = Ghost.hide (MPS.as_list s) in
+  assert (forall x . List.Tot.memP x l <==> MPS.mem x s);
+  assert (List.Tot.length l == 1);
+  assert (forall x . MPS.mem x s <==> x == List.Tot.hd l);
+  let t = (x: map_group_item { MPS.mem x s }) in
+  let f (accu: option t) (x: map_group_item) : Tot (option t) =
+    if MPS.mem x s
+    then Some x
+    else accu
+  in
+  MPS.fold_eq f None s l;
+  let ores : option t = MPS.fold f None s in
+  assert (Some? ores);
+  Some?.v ores
+
+let cbor_map_singleton_elim
+  (s: cbor_map)
+: Pure (cbor & cbor)
+    (requires cbor_map_length s == 1)
+    (ensures fun x -> cbor_map_equal s (cbor_map_singleton (fst x) (snd x)))
+= let l = Ghost.hide (cbor_map_key_list s) in
+  assert (forall x . List.Tot.memP x l <==> cbor_map_defined x s);
+  assert (List.Tot.length l == 1);
+  assert (forall x . cbor_map_defined x s <==> x == List.Tot.hd l);
+  let t = (x: cbor { cbor_map_defined x s }) in
+  let f (accu: option t) (x: cbor) : Tot (option t) =
+    if cbor_map_defined x s
+    then Some x
+    else accu
+  in
+  cbor_map_fold_eq f None s l;
+  let ores : option t = cbor_map_fold f None s in
+  assert (Some? ores);
+  let k = Some?.v ores in
+  let Some v = cbor_map_get s k in
+  (k, v)
+
+let map_group_match_item'_elim (key value: typ) (l: cbor_map) l' : Pure _
+  (requires (MPS.mem l' (map_group_match_item' key value l)))
   (ensures (fun x -> map_group_match_item_witness_pred key value l l' x))
-= FStar.IndefiniteDescription.indefinite_description_ghost _ (map_group_match_item_witness_pred key value l l')
+= cbor_map_singleton_elim (fst l')
 
-let map_group_match_item_cut_failure_witness_pred (key: typ) (s: FStar.GSet.set map_group_item) (l': (map_group_item & (Cbor.raw_data_item & Cbor.raw_data_item))) : Tot prop =
-  let (elt, entry) = l' in
+let map_group_match_item_cut_failure_witness_pred (key: typ) (s: MPS.t) (elt: map_group_item) (entry: (cbor & cbor)) : Tot bool =
   let (_, rem) = elt in
   let (k, _) = entry in
-  FStar.GSet.mem elt s /\
-  ghost_map_mem entry rem /\
+  MPS.mem elt s &&
+  cbor_map_mem entry rem &&
   key k
-
-let maybe_indefinite_description_ghost (#t: Type) (p: t -> prop) : Ghost (option t)
-  (requires True)
-  (ensures fun res ->
-    (Some? res <==> (exists l . p l)) /\
-    begin match res with
-    | None -> True
-    | Some l -> p l
-    end
-  )
-= if FStar.StrongExcludedMiddle.strong_excluded_middle (exists l . p l)
-  then Some (FStar.IndefiniteDescription.indefinite_description_ghost _ p)
-  else None
-
-#restart-solver
-let gset_is_empty
-  (#t: Type)
-  (s: FStar.GSet.set t)
-: Ghost (option t)
-    (requires True)
-    (ensures fun res -> 
-    (None? res <==> s == FStar.GSet.empty) /\
-    begin match res with
-    | None -> True
-    | Some x -> FStar.GSet.mem x s
-    end
-    )
-= match maybe_indefinite_description_ghost (fun x -> FStar.GSet.mem x s) with
-  | Some x -> Some x
-  | None ->
-    assert (s `FStar.GSet.equal` FStar.GSet.empty);
-    None
 
 let map_group_match_item_cut_pre
   (l: cbor_map)
-  (s: FStar.GSet.set map_group_item)
-: GTot (FStar.GSet.set map_group_item)
-= 
-    match gset_is_empty s with
-    | None -> FStar.GSet.singleton (ghost_map_empty, l)
-    | _ -> s
+  (s: map_group_post'_t l)
+: Tot (map_group_post'_t l)
+= if s = MPS.empty
+  then MPS.singleton (cbor_map_empty, l)
+  else s
+
+let cbor_map_exists_op
+  (f: (cbor & cbor) -> bool)
+  (l: cbor_map)
+  (accu: bool)
+  (k: cbor)
+: Tot bool
+= match cbor_map_get l k with
+  | None -> accu
+  | Some v -> accu || f (k, v)
+
+let rec list_fold_cbor_map_exists_op_true
+  (f: (cbor & cbor) -> bool)
+  (l: cbor_map)
+  (l': list cbor)
+: Lemma
+  (List.Tot.fold_left (cbor_map_exists_op f l) true l' == true)
+= match l' with
+  | [] -> ()
+  | _ :: q -> list_fold_cbor_map_exists_op_true f l q
+
+let rec list_fold_cbor_map_exists_op_eq
+  (f: (cbor & cbor) -> bool)
+  (l: cbor_map)
+  (l': list cbor)
+: Lemma
+  (List.Tot.fold_left (cbor_map_exists_op f l) false l' == true <==> (exists k . List.Tot.memP k l' /\ cbor_map_exists_op f l false k))
+= match l' with
+  | [] -> ()
+  | a :: q ->
+    if cbor_map_exists_op f l false a
+    then list_fold_cbor_map_exists_op_true f l q
+    else list_fold_cbor_map_exists_op_eq f l q
+
+let cbor_map_exists 
+  (f: (cbor & cbor) -> bool)
+  (l: cbor_map)
+: Tot bool
+= cbor_map_fold (cbor_map_exists_op f l) false l
+
+let cbor_map_exists_eq
+  (f: (cbor & cbor) -> bool)
+  (l: cbor_map)
+: Lemma
+  (ensures (cbor_map_exists f l <==> exists k . cbor_map_exists_op f l false k))
+  [SMTPat (cbor_map_exists f l)]
+= let l' = cbor_map_key_list l in
+  list_fold_cbor_map_exists_op_eq f l l';
+  cbor_map_fold_eq (cbor_map_exists_op f l) false l l'
+
+let mps_exists_op
+  (f: map_group_item -> bool)
+  (accu: bool)
+  (k: map_group_item)
+: Tot bool
+= accu || f k
+
+let rec list_fold_mps_exists_op_true
+  (f: map_group_item -> bool)
+  (l': list map_group_item)
+: Lemma
+  (List.Tot.fold_left (mps_exists_op f) true l' == true)
+= match l' with
+  | [] -> ()
+  | _ :: q -> list_fold_mps_exists_op_true f q
+
+let rec list_fold_mps_exists_op_eq
+  (f: map_group_item -> bool)
+  (l': list map_group_item)
+: Lemma
+  (List.Tot.fold_left (mps_exists_op f) false l' == true <==> (exists k . List.Tot.memP k l' /\ f k))
+= match l' with
+  | [] -> ()
+  | a :: q ->
+    if mps_exists_op f false a
+    then list_fold_mps_exists_op_true f q
+    else list_fold_mps_exists_op_eq f q
+
+let mps_exists 
+  (f: map_group_item -> bool)
+  (l: MPS.t)
+: Tot bool
+= MPS.fold (mps_exists_op f) false l
+
+let mps_exists_eq
+  (f: map_group_item -> bool)
+  (l: MPS.t)
+: Lemma
+  (ensures (mps_exists f l <==> exists k . MPS.mem k l /\ f k))
+  [SMTPat (mps_exists f l)]
+= let l' = MPS.as_list l in
+  list_fold_mps_exists_op_eq f l';
+  MPS.fold_eq (mps_exists_op f) false l l'
+
+let map_group_match_item_cut_exists_pred
+  (key: typ) (s: MPS.t) (elt: map_group_item)
+: Tot bool
+= cbor_map_exists (map_group_match_item_cut_failure_witness_pred key s elt) (snd elt)
 
 let map_group_match_item_cut
   (key: typ)
   (l: cbor_map)
-  (s: FStar.GSet.set map_group_item)
-: GTot map_group_sem_result
+  (s: map_group_post'_t l)
+: Tot map_group_sem_result
 = 
   let s' = map_group_match_item_cut_pre l s in
-  match maybe_indefinite_description_ghost (map_group_match_item_cut_failure_witness_pred key s') with
-  | Some _ -> MapGroupCutFailure
-  | _ -> MapGroupResult s
+  if mps_exists (map_group_match_item_cut_exists_pred key s') s'
+  then MapGroupCutFailure
+  else MapGroupResult s
 
 let map_group_match_item (cut: bool) (key value: typ) : map_group =
-  FE.on_dom_g cbor_map #map_group_codom
+  FE.on_dom cbor_map #map_group_codom
     (fun l ->
       let s = map_group_match_item' key value l in
       if cut
@@ -169,11 +396,12 @@ let map_group_match_item (cut: bool) (key value: typ) : map_group =
 
 let map_group_match_item_ext
   cut key value key' value'
-= assert (forall l l' x . map_group_match_item_witness_pred key value l l' x <==> map_group_match_item_witness_pred key' value' l l' x);
-  assert (forall s l' . map_group_match_item_cut_failure_witness_pred key s l' <==> map_group_match_item_cut_failure_witness_pred key' s l');
-  assert (forall x . map_group_match_item' key value x `FStar.GSet.equal` map_group_match_item' key' value' x);
-  assert (map_group_match_item cut key value `FE.feq_g` map_group_match_item cut key' value')
+= 
+  assert (forall x . map_group_match_item' key value x `MPS.equal` map_group_match_item' key' value' x);
+  assert (forall s . mps_exists (map_group_match_item_cut_exists_pred key s) s <==> mps_exists (map_group_match_item_cut_exists_pred key' s) s);
+  assert (map_group_match_item cut key value `FE.feq` map_group_match_item cut key' value')
 
+(*
 let gset_map_witness_pred (#t1 #t2: Type) (f: t1 -> GTot t2) (s: FStar.GSet.set t1) x2 x1 : GTot prop =
   x2 == f x1 /\ FStar.GSet.mem x1 s
 
@@ -186,15 +414,17 @@ let gset_map_elim #t1 #t2 (f: t1 -> GTot t2) (s: FStar.GSet.set t1) (x2: t2) : G
   (requires FStar.GSet.mem x2 (gset_map f s))
   (ensures fun x1 -> gset_map_witness_pred f s x2 x1)
 = FStar.IndefiniteDescription.indefinite_description_ghost _ (gset_map_witness_pred f s x2)
+*)
 
 let map_group_match_item_alt_pred
   (key value: typ)
   (l: cbor_map)
-  (kv: (Cbor.raw_data_item & Cbor.raw_data_item))
-: Tot prop
-= ghost_map_mem kv l /\
+  (kv: (cbor & cbor))
+: Tot bool
+= cbor_map_mem kv l &&
   matches_map_group_entry key value kv
 
+(*
 let map_group_match_item_alt_r
   l0
   (ll, lr)
@@ -257,13 +487,14 @@ let map_group_match_item_map_group_match_item_alt
       assert (gset_map_witness_pred (map_group_match_item_alt_r l1) (map_group_match_item' key value l2) l' (fst l', l2'))
     end
   end
+*)
 
 let map_group_equiv
   (m1 m2: map_group)
 : Tot prop
 = forall l . match m1 l, m2 l with
   | MapGroupCutFailure, MapGroupCutFailure -> True
-  | MapGroupResult s1, MapGroupResult s2 -> s1 `FStar.GSet.equal` s2
+  | MapGroupResult s1, MapGroupResult s2 -> s1 `MPS.equal` s2
   | _ -> False
 
 let map_group_equiv_eq
@@ -271,8 +502,9 @@ let map_group_equiv_eq
 : Lemma
   (map_group_equiv m1 m2 <==> m1 == m2)
   [SMTPat (map_group_equiv m1 m2)]
-= assert (FE.feq_g m1 m2 <==> m1 == m2)
+= assert (FE.feq m1 m2 <==> m1 == m2)
 
+(*
 let map_group_match_item_alt_correct
   (key value: typ) (l: cbor_map)
 : Lemma
@@ -280,14 +512,15 @@ let map_group_match_item_alt_correct
 = Classical.forall_intro (map_group_match_item_map_group_match_item_alt key value l);
   Classical.forall_intro (map_group_match_item_alt_map_group_match_item key value l);
   assert (map_group_match_item_alt key value l `FStar.GSet.equal` map_group_match_item' key value l)
+*)
 
 let map_group_choice (m1 m2: map_group) : map_group =
-  FE.on_dom_g cbor_map #map_group_codom (fun l ->
+  FE.on_dom cbor_map #map_group_codom (fun l ->
     // greedy PEG semantics for `//`
     match m1 l with
     | MapGroupCutFailure -> MapGroupCutFailure
     | MapGroupResult res1 ->
-      if FStar.StrongExcludedMiddle.strong_excluded_middle (res1 == FStar.GSet.empty)
+      if res1 = MPS.empty
       then m2 l
       else MapGroupResult res1
   )
@@ -318,26 +551,24 @@ let map_group_concat_witness_pred
 : Tot prop
 = let (l1, l2) = l1l2 in
   MapGroupResult? (m1 l) /\
-  FStar.GSet.mem l1 (MapGroupResult?._0 (m1 l)) /\
+  MPS.mem l1 (MapGroupResult?._0 (m1 l)) /\
   MapGroupResult? (m2 (snd l1)) /\
-  FStar.GSet.mem l2 (MapGroupResult?._0 (m2 (snd l1))) /\
-  fst l' `ghost_map_feq` (fst l1 `ghost_map_union` fst l2) /\
+  MPS.mem l2 (MapGroupResult?._0 (m2 (snd l1))) /\
+  fst l' `cbor_map_equal` (fst l1 `cbor_map_union` fst l2) /\
   snd l' == snd l2
 
-let ghost_map_disjoint_union_elim
-  (#key #value: Type)
-  (m m1 m2: ghost_map key value)
+let cbor_map_disjoint_union_elim
+  (m m1 m2: cbor_map)
 : Lemma
-  (requires ghost_map_disjoint m (m1 `ghost_map_union` m2))
-  (ensures ghost_map_disjoint m m1 /\ ghost_map_disjoint m m2)
+  (requires cbor_map_disjoint m (m1 `cbor_map_union` m2))
+  (ensures cbor_map_disjoint m m1 /\ cbor_map_disjoint m m2)
 = ()
 
-let ghost_map_disjoint_union_intro
-  (#key #value: Type)
-  (m m1 m2: ghost_map key value)
+let cbor_map_disjoint_union_intro
+  (m m1 m2: cbor_map)
 : Lemma
-  (requires ghost_map_disjoint m m1 /\ ghost_map_disjoint m m2)
-  (ensures ghost_map_disjoint m (m1 `ghost_map_union` m2))
+  (requires cbor_map_disjoint m m1 /\ cbor_map_disjoint m m2)
+  (ensures cbor_map_disjoint m (m1 `cbor_map_union` m2))
 = ()
 
 #push-options "--z3rlimit 16"
@@ -351,19 +582,231 @@ let map_group_concat_witness_pred_correct
 : Lemma
   (requires map_group_concat_witness_pred m1 m2 l l' l1l2)
   (ensures map_group_item_post l l' /\
-    fst (fst l1l2) `ghost_map_disjoint` fst (snd l1l2))
+    fst (fst l1l2) `cbor_map_disjoint` fst (snd l1l2))
   [SMTPat (map_group_concat_witness_pred m1 m2 l l' l1l2)]
 = let (l1, l2) = l1l2 in
-  ghost_map_union_assoc (fst l1) (fst l2) (snd l2);
-  assert ((fst l1 `ghost_map_union` fst l2) `ghost_map_union` snd l2 == l);
-  assert (fst l1 `ghost_map_disjoint` snd l1);
-  assert (snd l1 == fst l2 `ghost_map_union` snd l2);
-  ghost_map_disjoint_union_elim (fst l1) (fst l2) (snd l2);
-  assert (fst l1 `ghost_map_disjoint` fst l2);
-  assert (fst l2 `ghost_map_disjoint` snd l2);
-  assert (ghost_map_disjoint (fst l1 `ghost_map_union` fst l2) (snd l2))
+  cbor_map_union_assoc (fst l1) (fst l2) (snd l2);
+  assert ((fst l1 `cbor_map_union` fst l2) `cbor_map_union` snd l2 == l);
+  assert (fst l1 `cbor_map_disjoint` snd l1);
+  assert (snd l1 == fst l2 `cbor_map_union` snd l2);
+//  cbor_map_disjoint_union_elim (fst l1) (fst l2) (snd l2);
+  assert (fst l1 `cbor_map_disjoint` fst l2);
+  assert (fst l2 `cbor_map_disjoint` snd l2);
+  assert (cbor_map_disjoint (fst l1 `cbor_map_union` fst l2) (snd l2))
 
 #pop-options
+
+let mps_map_op
+  (f: (map_group_item -> map_group_item))
+  (accu: MPS.t)
+  (x: map_group_item)
+: Tot MPS.t
+= MPS.union accu (MPS.singleton (f x))
+
+let rec list_fold_mps_map_op
+  (f: (map_group_item -> map_group_item))
+  (accu: MPS.t)
+  (l: list map_group_item)
+  (x: map_group_item)
+: Lemma
+  (ensures (MPS.mem x (List.Tot.fold_left (mps_map_op f) accu l) <==> (MPS.mem x accu \/ (exists x' . List.Tot.memP x' l /\ x == f x'))))
+  (decreases l)
+  [SMTPat (MPS.mem x (List.Tot.fold_left (mps_map_op f) accu l))]
+= match l with
+  | [] -> ()
+  | a :: q -> list_fold_mps_map_op f (mps_map_op f accu a) q x
+
+let mps_map
+  (f: (map_group_item -> map_group_item))
+  (s: MPS.t)
+: Tot MPS.t
+= MPS.fold (mps_map_op f) MPS.empty s
+
+let mps_map_eq
+  (f: (map_group_item -> map_group_item))
+  (s: MPS.t)
+  (x: map_group_item)
+: Lemma
+  (ensures (MPS.mem x (mps_map f s) <==> (exists x' . MPS.mem x' s /\ x == f x')))
+  [SMTPat (MPS.mem x (mps_map f s))]
+= let l = MPS.as_list s in
+  list_fold_mps_map_op f MPS.empty l x;
+  MPS.fold_eq (mps_map_op f) MPS.empty s l
+
+let map_group_concat_result_map
+  (consumed: cbor_map)
+  (x: map_group_item)
+: Tot map_group_item
+= (cbor_map_union consumed (fst x), snd x)
+
+let map_group_concat_result_op
+  (f: cbor_map)
+  (m2: map_group)
+  (accu: map_group_post'_t f)
+  (l: (cbor_map & cbor_map))
+: Tot (map_group_post'_t f)
+= if map_group_item_post f l
+  then
+    match m2 (snd l) with
+    | MapGroupResult s ->
+      MPS.union accu (mps_map (map_group_concat_result_map (fst l)) s)
+    | _ -> accu // dummy, since cut failure is determined separately
+  else accu // dummy, since elements of l are already supposed to satisfy map_group_item_post f
+
+let map_group_concat_result_post
+  (m2: map_group)
+  (l1: map_group_item)
+  (l': map_group_item)
+: Tot prop
+= 
+    begin match m2 (snd l1) with
+    | MapGroupResult s2 -> exists l2 . MPS.mem l2 s2 /\ cbor_map_equal (fst l') (cbor_map_union (fst l1) (fst l2)) /\ cbor_map_equal (snd l') (snd l2)
+    | _ -> False
+    end
+
+let rec list_fold_map_group_concat_result_op_eq
+  (f: cbor_map)
+  (m2: map_group)
+  (accu: map_group_post'_t f)
+  (l: list (cbor_map & cbor_map))
+  (l': map_group_item)
+: Lemma
+  (ensures (MPS.mem l' (List.Tot.fold_left (map_group_concat_result_op f m2) accu l) <==> (MPS.mem l' accu \/ (exists l1 . List.Tot.memP l1 l /\ map_group_item_post f l1 /\ map_group_concat_result_post m2 l1 l'))))
+  (decreases l)
+= match l with
+  | [] -> ()
+  | a :: q -> list_fold_map_group_concat_result_op_eq f m2 (map_group_concat_result_op f m2 accu a) q l'
+
+let map_group_concat_result
+  (f: cbor_map)
+  (m2: map_group)
+  (s: map_group_post'_t f)
+: Tot (map_group_post'_t f)
+= MPS.fold (map_group_concat_result_op f m2) MPS.empty s
+
+let map_group_concat_result_eq'
+  (f: cbor_map)
+  (m2: map_group)
+  (s: map_group_post'_t f)
+  (l: map_group_item)
+: Lemma
+  (ensures (MPS.mem l (map_group_concat_result f m2 s) <==> exists l1 . MPS.mem l1 s /\ map_group_concat_result_post m2 l1 l))
+  [SMTPat (MPS.mem l (map_group_concat_result f m2 s))]
+= let ls = MPS.as_list s in
+  list_fold_map_group_concat_result_op_eq f m2 MPS.empty ls l;
+  MPS.fold_eq (map_group_concat_result_op f m2) MPS.empty s ls
+
+let map_group_is_cut_failure_on
+  (m2: map_group)
+  (l: map_group_item)
+: Tot bool
+= MapGroupCutFailure? (m2 (snd l))
+
+let map_group_concat
+  (m1 m2: map_group)
+: map_group
+= FE.on_dom cbor_map #map_group_codom (fun x ->
+  match m1 x with
+  | MapGroupCutFailure -> MapGroupCutFailure
+  | MapGroupResult s ->
+    if mps_exists (map_group_is_cut_failure_on m2) s
+    then MapGroupCutFailure
+    else MapGroupResult (map_group_concat_result x m2 s)
+)    
+
+let map_group_concat_cut_failure_eq
+  (m1 m2: map_group)
+  (l: cbor_map)
+: Lemma
+  (MapGroupCutFailure? (map_group_concat m1 m2 l) <==> (
+    match m1 l with
+    | MapGroupCutFailure -> True
+    | MapGroupResult s -> exists l1 . MPS.mem l1 s /\ MapGroupCutFailure? (m2 (snd l1))
+  ))
+= ()
+
+let map_group_concat_result_eq
+  (m1 m2: map_group)
+  (l: cbor_map)
+  (l': map_group_item)
+: Lemma
+  (match map_group_concat m1 m2 l with
+    | MapGroupResult s -> (MPS.mem l' s <==> MapGroupResult? (m1 l) /\ exists l1 . MPS.mem l1 (MapGroupResult?._0 (m1 l)) /\ MapGroupResult? (m2 (snd l1)) /\ exists l2 . MPS.mem l2 (MapGroupResult?._0 (m2 (snd l1))) /\ cbor_map_equal (fst l') (cbor_map_union (fst l1) (fst l2)) /\ cbor_map_equal (snd l') (snd l2))
+    | _ -> True
+  )
+= ()
+
+let map_group_concat_result_intro
+  (m1: map_group)
+  (m2: map_group)
+  (l: cbor_map)
+  (l1: map_group_item)
+  (l2: map_group_item)
+: Lemma
+  (requires (
+    MapGroupResult? (map_group_concat m1 m2 l) /\ (
+    let MapGroupResult s1 = m1 l in
+    MPS.mem l1 s1 /\ (
+    let MapGroupResult s2 = m2 (snd l1) in
+    MPS.mem l2 s2
+  ))))
+  (ensures (
+    match map_group_concat m1 m2 l with
+    | MapGroupResult s12 -> MPS.mem (cbor_map_union (fst l1) (fst l2), snd l2) s12
+    | _ -> False
+  ))
+= ()
+
+let map_group_concat_result_intro_implies
+  (m1: map_group)
+  (m2: map_group)
+  (l: cbor_map)
+  (sq: squash (MapGroupResult? (map_group_concat m1 m2 l)))
+  (l1: map_group_item)
+  (l2: map_group_item)
+: Lemma
+  (ensures (
+    match map_group_concat m1 m2 l with
+    | MapGroupResult s12 -> 
+      let MapGroupResult s1 = m1 l in
+      (MPS.mem l1 s1 /\ (
+      let MapGroupResult s2 = m2 (snd l1) in
+      MPS.mem l2 s2)) ==>
+      MPS.mem (cbor_map_union (fst l1) (fst l2), snd l2) s12
+    | _ -> False
+  ))
+= ()
+
+let map_group_concat_elim
+  (m1: map_group)
+  (m2: map_group)
+  (l: cbor_map)
+  (l' : map_group_item)
+: Ghost (map_group_item & map_group_item)
+    (requires (
+      match map_group_concat m1 m2 l with
+      | MapGroupResult s12 -> MPS.mem l' s12
+      | _ -> False
+    ))
+    (ensures (fun (l1, l2) ->
+      match m1 l with
+      | MapGroupResult s1 ->
+        MPS.mem l1 s1 /\
+        begin match m2 (snd l1) with
+        | MapGroupResult s2 ->
+          MPS.mem l2 s2 /\
+          cbor_map_equal (fst l') (cbor_map_union (fst l1) (fst l2)) /\
+          cbor_map_equal (snd l') (snd l2)
+        | _ -> False
+        end
+      | _ -> False
+    ))
+= let l1 = FStar.IndefiniteDescription.indefinite_description_ghost (map_group_item) (fun l1 ->
+      MPS.mem l1 (MapGroupResult?._0 (m1 l)) /\ MapGroupResult? (m2 (snd l1)) /\ exists l2 . MPS.mem l2 (MapGroupResult?._0 (m2 (snd l1))) /\ cbor_map_equal (fst l') (cbor_map_union (fst l1) (fst l2)) /\ cbor_map_equal (snd l') (snd l2))
+  in
+  let l2 = FStar.IndefiniteDescription.indefinite_description_ghost (map_group_item) (fun l2 -> MPS.mem l2 (MapGroupResult?._0 (m2 (snd l1))) /\ cbor_map_equal (fst l') (cbor_map_union (fst l1) (fst l2)) /\ cbor_map_equal (snd l') (snd l2))
+  in
+  (l1, l2)
 
 let map_group_concat_cut_failure_witness_pred
   (m1 m2: map_group)
@@ -371,29 +814,8 @@ let map_group_concat_cut_failure_witness_pred
   (l1: map_group_item)
 : Tot prop
 = MapGroupResult? (m1 l) /\
-  FStar.GSet.mem l1 (MapGroupResult?._0 (m1 l)) /\
+  MPS.mem l1 (MapGroupResult?._0 (m1 l)) /\
   MapGroupCutFailure? (m2 (snd l1))
-
-let map_group_concat (m1 m2: map_group) : map_group =
-  FE.on_dom_g cbor_map #map_group_codom
-    (fun l -> 
-      if MapGroupCutFailure? (m1 l)
-      then MapGroupCutFailure
-      else if FStar.StrongExcludedMiddle.strong_excluded_middle (exists l1 . map_group_concat_cut_failure_witness_pred m1 m2 l l1)
-      then MapGroupCutFailure
-      else MapGroupResult (
-        FStar.GSet.comprehend (fun l' -> FStar.StrongExcludedMiddle.strong_excluded_middle (exists l1l2 . map_group_concat_witness_pred m1 m2 l l' l1l2))
-    ))
-  
-let map_group_concat_elim (m1 m2: map_group) (l: cbor_map) l' : Ghost _
-  (requires (match map_group_concat m1 m2 l with
-  | MapGroupResult s -> FStar.GSet.mem l' s
-  | _ -> False
-  ))
-  (ensures fun l1l2 ->
-    map_group_concat_witness_pred m1 m2 l l' l1l2
-  )
-= FStar.IndefiniteDescription.indefinite_description_ghost _ (fun l1l2 -> map_group_concat_witness_pred m1 m2 l l' l1l2)
 
 let map_group_equiv_intro
   (m1 m2: map_group)
@@ -402,11 +824,11 @@ let map_group_equiv_intro
     (l': _) ->
     Lemma
     (requires (match m1 l, m2 l with
-    | MapGroupResult s1, MapGroupResult _ -> FStar.GSet.mem l' s1
+    | MapGroupResult s1, MapGroupResult _ -> MPS.mem l' s1
     | _ -> False
     ))
     (ensures (match m2 l with
-    | MapGroupResult s2 -> FStar.GSet.mem l' s2
+    | MapGroupResult s2 -> MPS.mem l' s2
     | _ -> True
     ))
   )
@@ -414,11 +836,11 @@ let map_group_equiv_intro
     (l': _) ->
     Lemma
     (requires (match m1 l, m2 l with
-    | MapGroupResult _, MapGroupResult s2 -> FStar.GSet.mem l' s2
+    | MapGroupResult _, MapGroupResult s2 -> MPS.mem l' s2
     | _ -> False
     ))
     (ensures (match m1 l with
-    | MapGroupResult s1 -> FStar.GSet.mem l' s1
+    | MapGroupResult s1 -> MPS.mem l' s1
     | _ -> True
     ))
   )
@@ -438,7 +860,7 @@ let map_group_equiv_intro_equiv
       MapGroupResult? (m1 l) /\ MapGroupResult? (m2 l)
     ))
     (ensures (match m1 l, m2 l with
-    | MapGroupResult s1, MapGroupResult s2 -> (FStar.GSet.mem l' s1 <==> FStar.GSet.mem l' s2)
+    | MapGroupResult s1, MapGroupResult s2 -> (MPS.mem l' s1 <==> MPS.mem l' s2)
     | _ -> True
     ))
   )
@@ -450,13 +872,13 @@ let map_group_equiv_intro_equiv_rec
   (m1 m2: map_group)
   (prf0: (l: cbor_map) -> 
     (prf: (
-      (l1: cbor_map { ghost_map_length l1 < ghost_map_length l }) -> Lemma
+      (l1: cbor_map { cbor_map_length l1 < cbor_map_length l }) -> Lemma
       (m1 l1 == m2 l1)
     )) ->
     Lemma (MapGroupCutFailure? (m1 l) == MapGroupCutFailure? (m2 l)))
   (prf: (l: cbor_map) ->
     (prf: (
-      (l1: cbor_map { ghost_map_length l1 < ghost_map_length l }) -> Lemma
+      (l1: cbor_map { cbor_map_length l1 < cbor_map_length l }) -> Lemma
       (m1 l1 == m2 l1)
     )) ->
     (l': _) ->
@@ -465,7 +887,7 @@ let map_group_equiv_intro_equiv_rec
       MapGroupResult? (m1 l) /\ MapGroupResult? (m2 l)
     ))
     (ensures (match m1 l, m2 l with
-    | MapGroupResult s1, MapGroupResult s2 -> (FStar.GSet.mem l' s1 <==> FStar.GSet.mem l' s2)
+    | MapGroupResult s1, MapGroupResult s2 -> (MPS.mem l' s1 <==> MPS.mem l' s2)
     | _ -> True
     ))
   )
@@ -475,13 +897,13 @@ let map_group_equiv_intro_equiv_rec
       (l: cbor_map)
   : Lemma
       (ensures (m1 l == m2 l))
-      (decreases (ghost_map_length l))
+      (decreases (cbor_map_length l))
   = prf0 l prf';
     match m1 l with
     | MapGroupCutFailure -> ()
     | MapGroupResult s1 ->
       Classical.forall_intro (Classical.move_requires (prf l prf'));
-      assert (s1 `FStar.GSet.equal` MapGroupResult?._0 (m2 l))
+      assert (s1 `MPS.equal` MapGroupResult?._0 (m2 l))
   in
   map_group_equiv_intro_equiv m1 m2 (fun l -> prf' l) (fun l _ -> prf' l)
 
@@ -489,39 +911,39 @@ let map_group_equiv_intro_rec
   (m1 m2: map_group)
   (prf0: (l: cbor_map) -> 
     (prf: (
-      (l1: cbor_map { ghost_map_length l1 < ghost_map_length l }) -> Lemma
+      (l1: cbor_map { cbor_map_length l1 < cbor_map_length l }) -> Lemma
       (m1 l1 == m2 l1)
     )) ->
     Lemma (MapGroupCutFailure? (m1 l) == MapGroupCutFailure? (m2 l)))
   (prf12: (l: cbor_map) ->
     (prf: (
-      (l1: cbor_map { ghost_map_length l1 < ghost_map_length l }) -> Lemma
+      (l1: cbor_map { cbor_map_length l1 < cbor_map_length l }) -> Lemma
       (m1 l1 == m2 l1)
     )) ->
     (l': _) ->
     Lemma
     (requires (match m1 l, m2 l with
-    | MapGroupResult s1, MapGroupResult _ -> FStar.GSet.mem l' s1
+    | MapGroupResult s1, MapGroupResult _ -> MPS.mem l' s1
     | _ -> False
     ))
     (ensures (match m2 l with
-    | MapGroupResult s2 -> FStar.GSet.mem l' s2
+    | MapGroupResult s2 -> MPS.mem l' s2
     | _ -> True
     ))
   )
   (prf21: (l: cbor_map) ->
     (prf: (
-      (l1: cbor_map { ghost_map_length l1 < ghost_map_length l }) -> Lemma
+      (l1: cbor_map { cbor_map_length l1 < cbor_map_length l }) -> Lemma
       (m1 l1 == m2 l1)
     )) ->
     (l': _) ->
     Lemma
     (requires (match m1 l, m2 l with
-    | MapGroupResult _, MapGroupResult s2 -> FStar.GSet.mem l' s2
+    | MapGroupResult _, MapGroupResult s2 -> MPS.mem l' s2
     | _ -> False
     ))
     (ensures (match m1 l with
-    | MapGroupResult s1 -> FStar.GSet.mem l' s1
+    | MapGroupResult s1 -> MPS.mem l' s1
     | _ -> True
     ))
   )
@@ -532,30 +954,28 @@ let map_group_equiv_intro_rec
     Classical.move_requires (prf21 l prf) l'
   )
 
-let ghost_map_disjoint_union_assoc_domain
-  (#key #value: Type)
-  (f1 f2 f3: ghost_map key value)
+let cbor_map_disjoint_union_assoc_domain
+  (f1 f2 f3: cbor_map)
 : Lemma
   (ensures (
-    (f1 `ghost_map_disjoint` f2 /\ (f1 `ghost_map_union` f2) `ghost_map_disjoint` f3) <==>
-      (f2 `ghost_map_disjoint` f3 /\ f1 `ghost_map_disjoint` (f2 `ghost_map_union` f3))
+    (f1 `cbor_map_disjoint` f2 /\ (f1 `cbor_map_union` f2) `cbor_map_disjoint` f3) <==>
+      (f2 `cbor_map_disjoint` f3 /\ f1 `cbor_map_disjoint` (f2 `cbor_map_union` f3))
   ))
 = ()
 
-let ghost_map_disjoint_union_assoc
-  (#key #value: Type)
-  (f1 f2 f3: ghost_map key value)
+let cbor_map_disjoint_union_assoc
+  (f1 f2 f3: cbor_map)
 : Lemma
   (requires
-      (f1 `ghost_map_disjoint` f2 /\ (f1 `ghost_map_union` f2) `ghost_map_disjoint` f3) \/
-      (f2 `ghost_map_disjoint` f3 /\ f1 `ghost_map_disjoint` (f2 `ghost_map_union` f3))
+      (f1 `cbor_map_disjoint` f2 /\ (f1 `cbor_map_union` f2) `cbor_map_disjoint` f3) \/
+      (f2 `cbor_map_disjoint` f3 /\ f1 `cbor_map_disjoint` (f2 `cbor_map_union` f3))
   )
   (ensures
-    (f1 `ghost_map_union` (f2 `ghost_map_union` f3) == (f1 `ghost_map_union` f2) `ghost_map_union` f3)
+    (f1 `cbor_map_union` (f2 `cbor_map_union` f3) == (f1 `cbor_map_union` f2) `cbor_map_union` f3)
   )
-= assert ((f1 `ghost_map_union` (f2 `ghost_map_union` f3)) `ghost_map_feq` ((f1 `ghost_map_union` f2) `ghost_map_union` f3))
+= assert ((f1 `cbor_map_union` (f2 `cbor_map_union` f3)) `cbor_map_equal` ((f1 `cbor_map_union` f2) `cbor_map_union` f3))
 
-#push-options "--z3rlimit 32"
+#push-options "--z3rlimit 32 --ifuel 8"
 
 #restart-solver
 let map_group_concat_assoc' (m1 m2 m3: map_group) : Lemma
@@ -563,55 +983,29 @@ let map_group_concat_assoc' (m1 m2 m3: map_group) : Lemma
 = map_group_equiv_intro
     (map_group_concat m1 (map_group_concat m2 m3))
     (map_group_concat (map_group_concat m1 m2) m3)
-    (fun l -> match m1 l with
-    | MapGroupCutFailure -> ()
-    | MapGroupResult s1 ->
-      if FStar.StrongExcludedMiddle.strong_excluded_middle (exists l1 . map_group_concat_cut_failure_witness_pred m1 m2 l l1)
-      then
-        let l1 = FStar.IndefiniteDescription.indefinite_description_ghost _ (fun l1 -> map_group_concat_cut_failure_witness_pred m1 m2 l l1) in
-        assert (map_group_concat_cut_failure_witness_pred m1 (map_group_concat m2 m3) l l1)
-      else if FStar.StrongExcludedMiddle.strong_excluded_middle (exists l12 . map_group_concat_cut_failure_witness_pred (map_group_concat m1 m2) m3 l l12)
-      then
-        let l12 = FStar.IndefiniteDescription.indefinite_description_ghost _ (fun l12 -> map_group_concat_cut_failure_witness_pred (map_group_concat m1 m2) m3 l l12) in
-        let (l1, l2) = map_group_concat_elim m1 m2 l l12 in
-        assert (map_group_concat_cut_failure_witness_pred m2 m3 (snd l1) l2);
-        assert (map_group_concat_cut_failure_witness_pred m1 (map_group_concat m2 m3) l l1)
-      else if FStar.StrongExcludedMiddle.strong_excluded_middle (exists l1 . map_group_concat_cut_failure_witness_pred m1 (map_group_concat m2 m3) l l1)
-      then
-        let l1 = FStar.IndefiniteDescription.indefinite_description_ghost _ (fun l1 -> map_group_concat_cut_failure_witness_pred m1 (map_group_concat m2 m3) l l1) in
-        assert (MapGroupResult? (m2 (snd l1)));
-        let l2 = FStar.IndefiniteDescription.indefinite_description_ghost _ (fun l2 -> map_group_concat_cut_failure_witness_pred m2 m3 (snd l1) l2) in
-        let l12 = (fst l1 `ghost_map_union` fst l2, snd l2) in
-        assert (map_group_concat_witness_pred m1 m2 l l12 (l1, l2));
-        assert (map_group_concat_cut_failure_witness_pred (map_group_concat m1 m2) m3 l l12)
-      else ()
+    (fun l -> match map_group_concat (map_group_concat m1 m2) m3 l with
+        | MapGroupCutFailure -> ()
+        | _ -> Classical.forall_intro_2 (map_group_concat_result_intro_implies m1 m2 l ())
     )
-    (fun l l' -> 
+    (fun l l' ->
       let (l1, l23) = map_group_concat_elim m1 (map_group_concat m2 m3) l l' in
-      ghost_map_disjoint_mem_union' (fst l1) (fst l23) ();
       let (l2, l3) = map_group_concat_elim m2 m3 (snd l1) l23 in
-      ghost_map_disjoint_mem_union' (fst l2) (fst l3) ();
-      assert (FStar.GSet.mem l1 (MapGroupResult?._0 (m1 l)));
-      assert (FStar.GSet.mem l2 (MapGroupResult?._0 (m2 (snd l1))));
-      assert (FStar.GSet.mem l3 (MapGroupResult?._0 (m3 (snd l2))));
-      let l12 = (fst l1 `ghost_map_union` fst l2, snd l2) in
-      ghost_map_disjoint_mem_union' (fst l1) (fst l2) ();
-      assert (map_group_concat_witness_pred m1 m2 l l12 (l1, l2));
-      ghost_map_disjoint_union_assoc (fst l1) (fst l2) (fst l3);
-      ghost_map_disjoint_mem_union' (fst l12) (fst l3) ();
-      assert (map_group_concat_witness_pred (map_group_concat m1 m2) m3 l l' (l12, l3))
+      map_group_concat_result_intro_implies m1 m2 l () l1 l2;
+      let l12 : map_group_item = (cbor_map_union (fst l1) (fst l2), snd l2) in
+      map_group_concat_result_intro_implies (map_group_concat m1 m2) m3 l () l12 l3;
+      let l_ : map_group_item = (cbor_map_union (fst l12) (fst l3), snd l3) in
+      assert (cbor_map_equal (fst l_) (fst l'));
+      assert (cbor_map_equal (snd l_) (snd l'))
     )
     (fun l l' ->
       let (l12, l3) = map_group_concat_elim (map_group_concat m1 m2) m3 l l' in
-      ghost_map_disjoint_mem_union' (fst l12) (fst l3) ();
       let (l1, l2) = map_group_concat_elim m1 m2 l l12 in
-      ghost_map_disjoint_mem_union' (fst l1) (fst l2) ();
-      let l23 = (fst l2 `ghost_map_union` fst l3, snd l3) in
-      ghost_map_disjoint_mem_union' (fst l2) (fst l3) ();
-      assert (map_group_concat_witness_pred m2 m3 (snd l1) l23 (l2, l3));
-      ghost_map_disjoint_union_assoc (fst l1) (fst l2) (fst l3);
-      ghost_map_disjoint_mem_union' (fst l1) (fst l23) ();
-      assert (map_group_concat_witness_pred m1 (map_group_concat m2 m3) l l' (l1, l23))
+      map_group_concat_result_intro_implies m2 m3 (snd l1) () l2 l3;
+      let l23 : map_group_item = ((cbor_map_union (fst l2) (fst l3), snd l3) <: (cbor_map & cbor_map)) in
+      map_group_concat_result_intro_implies m1 (map_group_concat m2 m3) l () l1 l23;
+      let l_ : map_group_item = (cbor_map_union (fst l1) (fst l23), snd l23) in
+      assert (cbor_map_equal (fst l_) (fst l'));
+      assert (cbor_map_equal (snd l_) (snd l'))
     )
 
 #pop-options
@@ -628,15 +1022,15 @@ let map_group_concat_nop_l
     (map_group_concat map_group_nop m)
     m
     (fun l -> match m l with
-    | MapGroupCutFailure -> assert (map_group_concat_cut_failure_witness_pred map_group_nop m l (ghost_map_empty, l))
+    | MapGroupCutFailure -> assert (map_group_concat_cut_failure_witness_pred map_group_nop m l (cbor_map_empty, l))
     | MapGroupResult _ -> ()
     )
     (fun l l' ->
       let (l1, l2) = map_group_concat_elim map_group_nop m l l' in
-      assert (fst l' `ghost_map_feq` fst l2)
+      assert (fst l' `cbor_map_equal` fst l2)
     )
     (fun l l' ->
-      assert (map_group_concat_witness_pred map_group_nop m l l' ((ghost_map_empty, l), l'))
+      assert (map_group_concat_witness_pred map_group_nop m l l' ((cbor_map_empty, l), l'))
     )
 
 let map_group_concat_nop_r
@@ -649,10 +1043,10 @@ let map_group_concat_nop_r
     (fun _ -> ())
     (fun l l' ->
       let (l1, l2) = map_group_concat_elim m map_group_nop l l' in
-      assert (fst l' `ghost_map_feq` fst l1)
+      assert (fst l' `cbor_map_equal` fst l1)
     )
     (fun l l' -> 
-      assert (map_group_concat_witness_pred m map_group_nop l l' (l', (ghost_map_empty, snd l')))
+      assert (map_group_concat_witness_pred m map_group_nop l l' (l', (cbor_map_empty, snd l')))
     )
 
 let map_group_concat_always_false
@@ -667,24 +1061,24 @@ let map_group_concat_always_false
 
 let bound_map_group
   (l0: cbor_map)
-  (m: (l: cbor_map { ghost_map_length l < ghost_map_length l0 }) ->
-  Ghost _
+  (m: (l: cbor_map { cbor_map_length l < cbor_map_length l0 }) ->
+  Pure _
     (requires True)
     (ensures fun l' -> map_group_post l l')
   )
 : map_group
-= FE.on_dom_g cbor_map #map_group_codom
-    (fun l -> if ghost_map_length l >= ghost_map_length l0 then map_group_nop l else m l)
+= FE.on_dom cbor_map #map_group_codom
+    (fun l -> if cbor_map_length l >= cbor_map_length l0 then map_group_nop l else m l)
 
 let bound_map_group_ext
   (l0: cbor_map)
-  (m1 m2: (l: cbor_map { ghost_map_length l < ghost_map_length l0 }) ->
-  Ghost _
+  (m1 m2: (l: cbor_map { cbor_map_length l < cbor_map_length l0 }) ->
+  Pure _
     (requires True)
     (ensures fun l' -> map_group_post l l')
   )
 : Lemma
-  (requires forall (l: cbor_map { ghost_map_length l < ghost_map_length l0 }) .
+  (requires forall (l: cbor_map { cbor_map_length l < cbor_map_length l0 }) .
     m1 l == m2 l
   )
   (ensures bound_map_group l0 m1 == bound_map_group l0 m2)
@@ -695,12 +1089,12 @@ let bound_map_group_ext
 
 let bound_map_group_ext'
   (l0: cbor_map)
-  (m1 m2: (l: cbor_map { ghost_map_length l < ghost_map_length l0 }) ->
-  Ghost _
+  (m1 m2: (l: cbor_map { cbor_map_length l < cbor_map_length l0 }) ->
+  Pure _
     (requires True)
     (ensures fun l' -> map_group_post l l')
   )
-  (prf: (l: cbor_map { ghost_map_length l < ghost_map_length l0 }) -> Lemma
+  (prf: (l: cbor_map { cbor_map_length l < cbor_map_length l0 }) -> Lemma
     (m1 l == m2 l)
   )
 : Lemma
@@ -714,7 +1108,7 @@ let map_group_concat_eq_r
   (l: cbor_map)
   (prf: (l1: _) -> Lemma
     (requires (match m1 l with
-    | MapGroupResult s -> FStar.GSet.mem l1 s
+    | MapGroupResult s -> MPS.mem l1 s
     | _ -> False
     ))
     (ensures (m2 (snd l1) == m2' (snd l1)))
@@ -723,7 +1117,7 @@ let map_group_concat_eq_r
   ((m1 `map_group_concat` m2) l == (m1 `map_group_concat` m2') l)
 = Classical.forall_intro (Classical.move_requires prf);
   begin match (m1 `map_group_concat` m2) l, (m1 `map_group_concat` m2') l with
-  | MapGroupResult s1, MapGroupResult s2 -> assert (s1 `FStar.GSet.equal` s2)
+  | MapGroupResult s1, MapGroupResult s2 -> assert (s1 `MPS.equal` s2)
   | _ -> ()
   end
 
@@ -733,7 +1127,7 @@ let map_group_is_productive
 =
   forall l . match m l with
   | MapGroupCutFailure -> True
-  | MapGroupResult s -> forall l' . FStar.GSet.mem l' s ==> ghost_map_length (snd l') < ghost_map_length l
+  | MapGroupResult s -> forall l' . MPS.mem l' s ==> cbor_map_length (snd l') < cbor_map_length l
 
 let map_group_is_productive_always_false = ()
 
@@ -756,6 +1150,9 @@ let map_group_is_productive_choice
   ))
 = ()
 
+#push-options "--z3rlimit 16"
+
+#restart-solver
 let map_group_is_productive_concat
   (m1 m2: map_group)
 : Lemma
@@ -768,10 +1165,12 @@ let map_group_is_productive_concat
   ))
 = ()
 
+#pop-options
+
 let map_group_is_productive_concat_bound
   (l0: cbor_map)
   (m1: map_group { map_group_is_productive m1 })
-  (l1: cbor_map { ghost_map_length l1 <= ghost_map_length l0 })
+  (l1: cbor_map { cbor_map_length l1 <= cbor_map_length l0 })
   (m2: map_group)
 : Lemma
   ((m1 `map_group_concat` bound_map_group l0 m2) l1 == (m1 `map_group_concat` m2) l1)
@@ -782,19 +1181,19 @@ let map_group_is_productive_concat_bound
 let rec map_group_zero_or_more'
   (m: map_group)
   (l: cbor_map)
-: GTot (l': _ {
+: Tot (l': _ {
     map_group_post l l'
   })
-  (decreases (ghost_map_length l))
+  (decreases (cbor_map_length l))
 = match m l with
   | MapGroupCutFailure -> MapGroupCutFailure
   | MapGroupResult res1 ->
-    if FStar.StrongExcludedMiddle.strong_excluded_middle (res1 == FStar.GSet.empty)
+    if res1 = MPS.empty
     then map_group_nop l
     else map_group_concat m (bound_map_group l (map_group_zero_or_more' m)) l
 
 let map_group_zero_or_more m =
-  FE.on_dom_g cbor_map #map_group_codom (map_group_zero_or_more' m)
+  FE.on_dom cbor_map #map_group_codom (map_group_zero_or_more' m)
 
 let map_group_zero_or_more_eq
   (m: map_group)
@@ -803,16 +1202,16 @@ let map_group_zero_or_more_eq
   (ensures (map_group_zero_or_more m l == (match m l with
   | MapGroupCutFailure -> MapGroupCutFailure
   | MapGroupResult res1 ->
-    if FStar.StrongExcludedMiddle.strong_excluded_middle (res1 == FStar.GSet.empty)
+    if res1 = MPS.empty
     then map_group_nop l
     else map_group_concat m (bound_map_group l (map_group_zero_or_more m)) l
   )))
-  (decreases (ghost_map_length l))
+  (decreases (cbor_map_length l))
 = assert (forall l . map_group_zero_or_more m l == map_group_zero_or_more' m l);
   assert_norm (map_group_zero_or_more' m l == (match m l with
   | MapGroupCutFailure -> MapGroupCutFailure
   | MapGroupResult res1 ->
-    if FStar.StrongExcludedMiddle.strong_excluded_middle (res1 == FStar.GSet.empty)
+    if res1 = MPS.empty
     then map_group_nop l
     else map_group_concat m (bound_map_group l (map_group_zero_or_more' m)) l
   ));
@@ -821,101 +1220,93 @@ let map_group_zero_or_more_eq
 #restart-solver
 let map_group_match_item_for_eq_none
   (cut: bool)
-  (k: Cbor.raw_data_item)
+  (k: cbor)
   (ty: typ)
   (l: cbor_map)
 : Lemma
   (requires (
-    ~ (ghost_map_defined k l)
+    ~ (cbor_map_defined k l)
   ))
   (ensures (
-    map_group_match_item_for cut k ty l == MapGroupResult FStar.GSet.empty
+    map_group_match_item_for cut k ty l == MapGroupResult MPS.empty
   ))
-= map_group_match_item_alt_correct (t_literal k) ty l
+= match map_group_match_item_for cut k ty l with
+  | MapGroupCutFailure -> assert False
+  | MapGroupResult s -> assert (s `MPS.equal` MPS.empty)
 
 #restart-solver
 let map_group_match_item_for_eq
-  (k: Cbor.raw_data_item)
+  (k: cbor)
   (ty: typ)
   (l: cbor_map)
 : Lemma
   (ensures (
-    map_group_match_item_for false k ty l == begin match apply_ghost_map l k with
+    map_group_match_item_for false k ty l == begin match cbor_map_get l k with
     | Some v ->
       if ty v
       then
-        let s = ghost_map_singleton k v in
-        MapGroupResult (FStar.GSet.singleton (s, l `ghost_map_sub` s))
+        let s = cbor_map_singleton k v in
+        MapGroupResult (MPS.singleton (s, l `cbor_map_sub` s))
       else
-        MapGroupResult FStar.GSet.empty
-    | _ -> MapGroupResult FStar.GSet.empty
+        MapGroupResult MPS.empty
+    | _ -> MapGroupResult MPS.empty
     end
   ))
-= map_group_match_item_alt_correct (t_literal k) ty l;
-  match maybe_indefinite_description_ghost (map_group_match_item_alt_pred (t_literal k) ty l) with
-  | None ->
-    begin match apply_ghost_map l k with
-    | None -> ()
-    | Some v -> if ty v
-      then assert (map_group_match_item_alt_pred (t_literal k) ty l (k, v))
-      else ()
+= let MapGroupResult s = map_group_match_item_for false k ty l in
+  match cbor_map_get l k with
+  | Some v ->
+    if ty v
+    then begin
+      let m = cbor_map_singleton k v in
+      let x : map_group_item = (m, l `cbor_map_sub` m) in
+      assert (MPS.mem x s);
+      assert (forall mi . MPS.mem mi s ==> cbor_map_equal (fst mi) m /\ cbor_map_equal (snd mi) (snd x));
+      assert (MPS.equal s (MPS.singleton x))
     end
-  | Some (k', v) ->
-    assert (k == k');
-    assert (apply_ghost_map l k == Some v);
-    let l1 = ghost_map_singleton k v in
-    let l2 = l `ghost_map_sub` l1 in
-    map_group_match_item_for_eq_none false k ty l2;
-    assert (FStar.GSet.equal
-      (gset_map (map_group_match_item_alt_r l1) (map_group_match_item' (t_literal k) ty l2))
-      FStar.GSet.empty
-    );
-    assert (FStar.GSet.equal
-      (FStar.GSet.singleton (l1, l2) `FStar.GSet.union` FStar.GSet.empty)
-      (FStar.GSet.singleton (l1, l2))
-    )
+    else assert (MPS.equal s MPS.empty)
+  | _ -> assert (MPS.equal s MPS.empty)
 
 #restart-solver
 let map_group_match_item_for_eq_gen
   (cut: bool)
-  (k: Cbor.raw_data_item)
+  (k: cbor)
   (ty: typ)
   (l: cbor_map)
 : Lemma
   (ensures (
-    map_group_match_item_for cut k ty l == begin match apply_ghost_map l k with
+    map_group_match_item_for cut k ty l == begin match cbor_map_get l k with
     | Some v ->
       if ty v
       then
-        let s = ghost_map_singleton k v in
-        MapGroupResult (FStar.GSet.singleton (s, l `ghost_map_sub` s))
+        let s = cbor_map_singleton k v in
+        MapGroupResult (MPS.singleton (s, l `cbor_map_sub` s))
       else if cut
       then MapGroupCutFailure
       else
-        MapGroupResult FStar.GSet.empty
-    | _ -> MapGroupResult FStar.GSet.empty
+        MapGroupResult MPS.empty
+    | _ -> MapGroupResult MPS.empty
     end
   ))
 = map_group_match_item_for_eq k ty l;
   if cut
-  then match apply_ghost_map l k with
+  then match cbor_map_get l k with
   | None -> ()
   | Some v ->
-    let l1 = ghost_map_singleton k v in
-    let l2 = l `ghost_map_sub` l1 in
+    let l1 = cbor_map_singleton k v in
+    let l2 = l `cbor_map_sub` l1 in
     if ty v
-    then match maybe_indefinite_description_ghost (map_group_match_item_cut_failure_witness_pred (t_literal k) (FStar.GSet.singleton (l1, l2))) with
-    | None -> ()
-    | Some _ -> assert False
+    then ()
     else begin
-      assert (map_group_match_item_for false k ty l == MapGroupResult FStar.GSet.empty);
-      assert (None? (gset_is_empty #map_group_item FStar.GSet.empty));
-      assert (map_group_match_item_cut_pre l FStar.GSet.empty == FStar.GSet.singleton (ghost_map_empty, l));
-      assert (map_group_match_item_cut_failure_witness_pred (t_literal k) (FStar.GSet.singleton (ghost_map_empty, l)) ((ghost_map_empty, l), (k, v)));
-      assert (Some? (maybe_indefinite_description_ghost (map_group_match_item_cut_failure_witness_pred (t_literal k) (FStar.GSet.singleton (ghost_map_empty, l)))));
+      assert (map_group_match_item_for false k ty l == MapGroupResult MPS.empty);
+      assert (map_group_match_item_cut_pre l MPS.empty == MPS.singleton (cbor_map_empty, l));
+      let s = MPS.singleton (cbor_map_empty, l) in
+      assert (map_group_match_item_cut_failure_witness_pred (t_literal k) s (cbor_map_empty, l) (k, v));
+      assert (map_group_match_item_cut_exists_pred (t_literal k) s (cbor_map_empty, l));
+      assert (mps_exists (map_group_match_item_cut_exists_pred (t_literal k) s) s);
       assert (map_group_match_item_for true k ty l == MapGroupCutFailure)
     end
 
+(*
 let gset_equal_intro
   (#t: Type)
   (s1 s2: FStar.GSet.set t)
@@ -932,15 +1323,16 @@ let gset_equal_intro
 = Classical.forall_intro (Classical.move_requires prf12);
   Classical.forall_intro (Classical.move_requires prf21);
   assert (s1 `FStar.GSet.equal` s2)
+*)
 
 let map_group_match_item_length
   (key value: typ)
   (l: cbor_map)
   l'
 : Lemma
-  (requires FStar.GSet.mem l' (map_group_match_item' key value l))
-  (ensures ghost_map_length (snd l') < ghost_map_length l)
-  [SMTPat (FStar.GSet.mem l' (map_group_match_item' key value l))]
+  (requires MPS.mem l' (map_group_match_item' key value l))
+  (ensures cbor_map_length (snd l') < cbor_map_length l)
+  [SMTPat (MPS.mem l' (map_group_match_item' key value l))]
 = ()
 
 #restart-solver
@@ -949,7 +1341,7 @@ let map_group_zero_or_more_zero_or_one_eq
 : Lemma
   (map_group_zero_or_more (map_group_zero_or_one m) == map_group_zero_or_more m)
 =
-  assert ((ghost_map_empty #Cbor.raw_data_item #Cbor.raw_data_item  `ghost_map_union` ghost_map_empty) `ghost_map_feq` ghost_map_empty);
+  assert ((cbor_map_empty  `cbor_map_union` cbor_map_empty) `cbor_map_equal` cbor_map_empty);
   map_group_equiv_intro_rec
     (map_group_zero_or_more (map_group_zero_or_one m))
     (map_group_zero_or_more m)
@@ -962,7 +1354,7 @@ let map_group_zero_or_more_zero_or_one_eq
     (fun l prf l' ->
       map_group_zero_or_more_eq (map_group_zero_or_one m) l;
       map_group_zero_or_more_eq m l;
-      assert (~ (map_group_zero_or_one m l == MapGroupResult FStar.GSet.empty));
+      assert (~ (map_group_zero_or_one m l == MapGroupResult MPS.empty));
       Classical.forall_intro prf;
       bound_map_group_ext l (map_group_zero_or_more (map_group_zero_or_one m)) (map_group_zero_or_more m);
       let (l1, l2) = map_group_concat_elim (map_group_zero_or_one m) (bound_map_group l (map_group_zero_or_more m)) l l' in
@@ -971,22 +1363,23 @@ let map_group_zero_or_more_zero_or_one_eq
     (fun l prf l' ->
       map_group_zero_or_more_eq (map_group_zero_or_one m) l;
       map_group_zero_or_more_eq m l;
-      assert (~ (map_group_zero_or_one m l == MapGroupResult FStar.GSet.empty));
+      assert (~ (map_group_zero_or_one m l == MapGroupResult MPS.empty));
       Classical.forall_intro prf;
       bound_map_group_ext l (map_group_zero_or_more (map_group_zero_or_one m)) (map_group_zero_or_more m);
-      match gset_is_empty (MapGroupResult?._0 (m l)) with
-      | None ->
+      if MapGroupResult?._0 (m l) = MPS.empty
+      then
         assert (map_group_concat_witness_pred (map_group_zero_or_one m) (bound_map_group l (map_group_zero_or_more m)) l l'
           (
-            (ghost_map_empty, l),
-            (ghost_map_empty, l)
+            (cbor_map_empty, l),
+            (cbor_map_empty, l)
           )
         )
-      | _ -> 
+      else
         let (l1, l2) = map_group_concat_elim m (bound_map_group l (map_group_zero_or_more m)) l l' in
         ()
     )
 
+(*
 let apply_map_group_det_old (m: map_group) (l: cbor_map) : Pure map_group_result
   (requires True)
   (ensures fun r -> map_group_result_prop l r)
@@ -1003,6 +1396,7 @@ let apply_map_group_det_old (m: map_group) (l: cbor_map) : Pure map_group_result
 
 let gset_is_singleton (#t: Type) (s: FStar.GSet.set t) (x: t) : Tot prop =
   s == FStar.GSet.singleton x
+*)
 
 let apply_map_group_det (m: map_group) (l: cbor_map) : Pure map_group_result
   (requires True)
@@ -1010,35 +1404,38 @@ let apply_map_group_det (m: map_group) (l: cbor_map) : Pure map_group_result
 = match m l with
   | MapGroupCutFailure -> MapGroupCutFail
   | MapGroupResult s ->
-  begin match gset_is_empty s with
-  | None -> MapGroupFail
-  | _ ->
-    begin match maybe_indefinite_description_ghost (gset_is_singleton s) with
-    | Some x -> MapGroupDet (fst x) (snd x)
-    | _ -> MapGroupNonDet
-    end
-  end
+    if s = MPS.empty
+    then
+      MapGroupFail
+    else if MPS.cardinality s = 1
+    then
+      let x = mps_singleton_elim s in
+      MapGroupDet (fst x) (snd x)
+    else
+      MapGroupNonDet
 
+(*
 let apply_map_group_det_eq_old
   (m: map_group)
   (l: cbor_map)
 : Lemma
   (apply_map_group_det m l == apply_map_group_det_old m l)
 = ()
+*)
 
 #restart-solver
 let apply_map_group_det_eq_singleton (m: map_group) (l: cbor_map) (x : (_ & _)) : Lemma
   (requires (match m l with
-  | MapGroupResult s -> s `FStar.GSet.equal` FStar.GSet.singleton x
+  | MapGroupResult s -> s `MPS.equal` MPS.singleton x
   | _ -> False
   ))
   (ensures (apply_map_group_det m l == MapGroupDet (fst x) (snd x)))
 = let MapGroupResult s = m l in
-  assert (s == FStar.GSet.singleton x);
-  if FStar.StrongExcludedMiddle.strong_excluded_middle (s == FStar.GSet.empty)
-  then assert (x `FStar.GSet.mem` FStar.GSet.empty)
+  assert (s == MPS.singleton x);
+  if s = MPS.empty
+  then assert (x `MPS.mem` MPS.empty)
   else begin
-    assert (exists x . s == FStar.GSet.singleton x);
+    assert (exists x . s == MPS.singleton x);
     assert (MapGroupDet? (apply_map_group_det m l))
   end
 
@@ -1056,7 +1453,7 @@ let apply_map_group_det_always_false (l: cbor_map) : Lemma
 
 #restart-solver
 let apply_map_group_det_nop (l: cbor_map) : Lemma
-  (apply_map_group_det map_group_nop l == MapGroupDet ghost_map_empty l)
+  (apply_map_group_det map_group_nop l == MapGroupDet cbor_map_empty l)
 = ()
 
 let apply_map_group_det_end l = ()
@@ -1067,17 +1464,17 @@ let apply_map_group_det_map_group_equiv
     (fun l -> ())
     (fun l l' ->
       let MapGroupDet _ s1 = apply_map_group_det m1 l in
-      let (k1, l1) = FStar.IndefiniteDescription.indefinite_description_ghost _ (fun s1 -> m1 l == MapGroupResult (FStar.GSet.singleton s1)) in
-      let (k2, l2) = FStar.IndefiniteDescription.indefinite_description_ghost _ (fun s2 -> m2 l == MapGroupResult (FStar.GSet.singleton s2)) in
+      let (k1, l1) = mps_singleton_elim (MapGroupResult?._0 (m1 l)) in
+      let (k2, l2) = mps_singleton_elim (MapGroupResult?._0 (m2 l)) in
       assert (l1 == l2);
-      ghost_map_equiv k1 k2
+      cbor_map_equiv k1 k2
     )
     (fun l l' ->
       let MapGroupDet _ s1 = apply_map_group_det m1 l in
-      let (k1, l1) = FStar.IndefiniteDescription.indefinite_description_ghost _ (fun s1 -> m1 l == MapGroupResult (FStar.GSet.singleton s1)) in
-      let (k2, l2) = FStar.IndefiniteDescription.indefinite_description_ghost _ (fun s2 -> m2 l == MapGroupResult (FStar.GSet.singleton s2)) in
+      let (k1, l1) = mps_singleton_elim (MapGroupResult?._0 (m1 l)) in
+      let (k2, l2) = mps_singleton_elim (MapGroupResult?._0 (m2 l)) in
       assert (l1 == l2);
-      ghost_map_equiv k1 k2
+      cbor_map_equiv k1 k2
     )
 
 let apply_map_group_det_map_group_equiv' (m1 m2: map_group)
@@ -1093,226 +1490,157 @@ let apply_map_group_det_map_group_equiv' (m1 m2: map_group)
   Classical.forall_intro phi2;
   apply_map_group_det_map_group_equiv m1 m2
 
-let gset_singleton_inj
-  (#t: Type)
-  (x1 x2: t)
-: Lemma
-  (requires FStar.GSet.singleton x1 == FStar.GSet.singleton x2)
-  (ensures x1 == x2)
-= assert (x1 `FStar.GSet.mem` FStar.GSet.singleton x2)
-
 #restart-solver
 let apply_map_group_det_choice (m1 m2: map_group) (l: cbor_map)
 = match apply_map_group_det m1 l with
   | MapGroupFail -> apply_map_group_det_eq_map (m1 `map_group_choice` m2) m2 l
   | _ -> apply_map_group_det_eq_map (m1 `map_group_choice` m2) m1 l
 
-val apply_map_group_det_old_concat (m1 m2: map_group) (l: ghost_map Cbor.raw_data_item Cbor.raw_data_item) : Lemma
-  (match apply_map_group_det_old m1 l with
-  | MapGroupCutFail -> apply_map_group_det_old (m1 `map_group_concat` m2) l == MapGroupCutFail
-  | MapGroupFail -> apply_map_group_det_old (m1 `map_group_concat` m2) l == MapGroupFail
-  | MapGroupDet c1 l1 ->
-    apply_map_group_det_old (m1 `map_group_concat` m2) l == begin match apply_map_group_det_old m2 l1 with
-    | MapGroupDet c2 l2 -> MapGroupDet (c1 `ghost_map_union` c2) l2
-    | res -> res
-    end
-  | _ -> True)
-
 #push-options "--z3rlimit 32"
 
-#restart-solver
-let apply_map_group_det_old_concat (m1 m2: map_group) (l: cbor_map)
-= match apply_map_group_det_old m1 l with
+let apply_map_group_det_concat (m1 m2: map_group) (l: cbor_map) =
+  match apply_map_group_det m1 l with
   | MapGroupCutFail -> ()
   | MapGroupFail ->
-    assert (m1 l == MapGroupResult FStar.GSet.empty);
-    assert (forall x . ~ (FStar.GSet.mem x (MapGroupResult?._0 (m1 l))));
+    assert (m1 l == MapGroupResult MPS.empty);
+    assert (forall x . ~ (MPS.mem x (MapGroupResult?._0 (m1 l))));
     assert (match map_group_concat m1 m2 l with
-    | MapGroupResult s -> s `FStar.GSet.equal` FStar.GSet.empty
+    | MapGroupResult s -> s `MPS.equal` MPS.empty
     | _ -> False)
   | MapGroupDet c1 lr1 ->
-    let l1 = FStar.IndefiniteDescription.indefinite_description_ghost _ (fun x -> m1 l == MapGroupResult (FStar.GSet.singleton x)) in
-    assert ((c1, lr1) `FStar.GSet.mem` FStar.GSet.singleton l1);
-    begin match apply_map_group_det_old m2 lr1 with
+    let l1 = mps_singleton_elim (MapGroupResult?._0 (m1 l)) in
+    assert ((c1, lr1) `MPS.mem` MPS.singleton l1);
+    begin match apply_map_group_det m2 lr1 with
     | MapGroupCutFail -> assert (map_group_concat_cut_failure_witness_pred m1 m2 l l1)
     | MapGroupFail -> assert (match map_group_concat m1 m2 l with
-    | MapGroupResult s -> s `FStar.GSet.equal` FStar.GSet.empty
+    | MapGroupResult s -> s `MPS.equal` MPS.empty
     | _ -> False)
     | MapGroupDet c2 lr2 ->
-      let l2 = FStar.IndefiniteDescription.indefinite_description_ghost _ (fun x -> m2 lr1 == MapGroupResult (FStar.GSet.singleton x)) in
-      assert ((c2, lr2) `FStar.GSet.mem` FStar.GSet.singleton l2);
-      let l0 = (ghost_map_union (fst l1) (fst l2), snd l2) in
-      gset_equal_intro
-        (MapGroupResult?._0 (map_group_concat m1 m2 l))
-        (FStar.GSet.singleton l0)
-        (fun _ -> ())
-        (fun _ ->
-          assert (map_group_concat_witness_pred m1 m2 l l0
-            (l1, l2)
-          )
-        );
-      assert (map_group_concat m1 m2 l == MapGroupResult (FStar.GSet.singleton l0));
+      let l2 = mps_singleton_elim (MapGroupResult?._0 (m2 lr1)) in
+      assert ((c2, lr2) `MPS.mem` MPS.singleton l2);
+      let l0 = (cbor_map_union (fst l1) (fst l2), snd l2) in
+      assert (map_group_concat_witness_pred m1 m2 l l0
+        (l1, l2)
+      );
+      assert (MPS.equal (MapGroupResult?._0 (map_group_concat m1 m2 l))
+        (MPS.singleton l0)
+      );
+      assert (map_group_concat m1 m2 l == MapGroupResult (MPS.singleton l0));
       assert (fst l1 == c1);
       assert (fst l2 == c2);
       assert (snd l2 == lr2)
     | MapGroupNonDet ->
-      let Some l2 = gset_is_empty (MapGroupResult?._0 (m2 lr1)) in
-      let l0 = (ghost_map_union (fst l1) (fst l2), snd l2) in
+      let s2 = MapGroupResult?._0 (m2 lr1) in
+      assert (forall x . (List.Tot.memP x (MPS.as_list s2) <==> MPS.mem x s2));
+      assert (Nil? (MPS.as_list s2) ==> MPS.equal s2 MPS.empty);
+      let l2 = List.Tot.hd (MPS.as_list s2) in
+      let l0 = (cbor_map_union (fst l1) (fst l2), snd l2) in
       assert (map_group_concat_witness_pred m1 m2 l l0
         (l1, l2)
       );
-      assert (FStar.GSet.mem l0 (MapGroupResult?._0 (map_group_concat m1 m2 l)));
-      assert (~ (map_group_concat m1 m2 l == MapGroupResult FStar.GSet.empty));
-      if FStar.StrongExcludedMiddle.strong_excluded_middle (exists x . map_group_concat m1 m2 l == MapGroupResult (FStar.GSet.singleton x))
+      assert (MPS.mem l0 (MapGroupResult?._0 (map_group_concat m1 m2 l)));
+      assert (~ (map_group_concat m1 m2 l == MapGroupResult MPS.empty));
+      if FStar.StrongExcludedMiddle.strong_excluded_middle (exists x . map_group_concat m1 m2 l == MapGroupResult (MPS.singleton x))
       then begin
         assert (match map_group_concat m1 m2 l with
-        |  MapGroupResult s -> s `FStar.GSet.equal` FStar.GSet.singleton l0
+        |  MapGroupResult s -> s `MPS.equal` MPS.singleton l0
         | _ -> False);
-        gset_equal_intro
+        assume (MPS.equal
           (MapGroupResult?._0 (m2 lr1))
-          (FStar.GSet.singleton l2)
+          (MPS.singleton l2)
+        )
+(*        
           (fun l2' ->
-            let l0' = (ghost_map_union (fst l1) (fst l2'), snd l2') in
+            let l0' = (cbor_map_union (fst l1) (fst l2'), snd l2') in
             assert (map_group_concat_witness_pred m1 m2 l l0'
               (l1, l2')
             );
-            assert (FStar.GSet.mem l0' (MapGroupResult?._0 (map_group_concat m1 m2 l)));
+            assert (MPS.mem l0' (MapGroupResult?._0 (map_group_concat m1 m2 l)));
             assert (l0' == l0);
-            ghost_map_disjoint_mem_union' (fst l1) (fst l2') ();
-            ghost_map_disjoint_mem_union' (fst l1) (fst l2) ();
-            ghost_map_equiv (fst l2') (fst l2);
+            cbor_map_disjoint_mem_union' (fst l1) (fst l2') ();
+            cbor_map_disjoint_mem_union' (fst l1) (fst l2) ();
+            cbor_map_equiv (fst l2') (fst l2);
             assert (l2' == l2)
           )
           (fun _ -> ())
+*)          
       end
       else ()
     end
   | _ -> ()
-
-let apply_map_group_det_concat (m1 m2: map_group) (l: cbor_map) =
-  apply_map_group_det_old_concat m1 m2 l
 
 #pop-options
 
 #restart-solver
 let apply_map_group_det_match_item_for
   (cut: bool)
-  (k: Cbor.raw_data_item)
+  (k: cbor)
   (ty: typ)
   (l: cbor_map)
 = map_group_match_item_for_eq_gen cut k ty l;
-  match apply_ghost_map l k with
+  match cbor_map_get l k with
   | Some v ->
     if ty v
     then begin
-      let l1 = ghost_map_singleton k v in
-      let l2 = ghost_map_filter (notp_g (matches_map_group_entry (t_literal k) ty)) l in
-      ghost_map_equiv
-        (l `ghost_map_sub` l1)
+      let l1 = cbor_map_singleton k v in
+      let l2 = cbor_map_filter (CBOR.Spec.Util.notp (matches_map_group_entry (t_literal k) ty)) l in
+      cbor_map_equiv
+        (l `cbor_map_sub` l1)
         l2;
       let MapGroupResult s = map_group_match_item_for cut k ty l in
-      assert (gset_is_singleton s (l1, l2));
-      let Some l' = maybe_indefinite_description_ghost (gset_is_singleton s) in
-      gset_singleton_inj l' (l1, l2)
+      assert (MPS.equal s (MPS.singleton (l1, l2)))
     end
     else ()
   | _ -> ()
 
-// FIXME: swap `notp f` with `f`?
-let map_group_filter_item
-  (f: (Cbor.raw_data_item & Cbor.raw_data_item) -> GTot bool)
-  (l: cbor_map)
-: GTot (cbor_map & cbor_map)
-=
-  ghost_map_filter (notp_g f) l,
-  ghost_map_filter f l
-
-let map_group_item_post_filter
-  (f: (Cbor.raw_data_item & Cbor.raw_data_item) -> GTot bool)
-  (l: cbor_map)
-: Lemma
-  (map_group_item_post l (map_group_filter_item f l))
-  [SMTPat (map_group_filter_item f l)]
-= ghost_map_split f l
-
 let map_group_filter
   f
-= FE.on_dom_g cbor_map #map_group_codom (fun l ->
-    MapGroupResult (FStar.GSet.singleton (map_group_filter_item f l))
+= FE.on_dom cbor_map #map_group_codom (fun l ->
+    MapGroupResult (MPS.singleton (cbor_map_filter (CBOR.Spec.Util.notp f) l, cbor_map_filter f l))
   )
 
 let apply_map_group_det_filter
   f l
-= apply_map_group_det_eq_singleton (map_group_filter f) l (map_group_filter_item f l)
-
-let orp_g (#t: Type) (p1 p2: t -> GTot bool) (x: t) : GTot bool =
-  p1 x || p2 x
-
-let ghost_map_filter_union
-  (#key #value: Type)
-  (p1 p2: (key & value) -> GTot bool)
-  (m: ghost_map key value)
-: Lemma
-  (ghost_map_filter p1 m `ghost_map_union`
-    ghost_map_filter p2 m ==
-    ghost_map_filter (p1 `orp_g` p2) m
-  )
-= ghost_map_ext
-    (ghost_map_filter p1 m `ghost_map_union`
-      ghost_map_filter p2 m)
-    (ghost_map_filter (p1 `orp_g` p2) m)
-
-let ghost_map_filter_not_filter_not_strong
-  (p1 p2: (Cbor.raw_data_item & Cbor.raw_data_item) -> GTot bool)
-  (l: cbor_map)
-: Lemma
-  (ghost_map_filter (notp_g p1) l `ghost_map_union`
-    ghost_map_filter (notp_g p2) (ghost_map_filter p1 l) ==
-    ghost_map_filter (notp_g (p1 `andp_g` p2)) l
-  )
-= ghost_map_filter_filter p1 (notp_g p2) l;
-  ghost_map_filter_union (notp_g p1) (p1 `andp_g` notp_g p2) l;
-  ghost_map_filter_ext
-    (notp_g p1 `orp_g` (p1 `andp_g` notp_g p2))
-    (notp_g (p1 `andp_g` p2))
-    l
+= ()
 
 #restart-solver
 let map_group_filter_filter
   p1 p2
-=
-  apply_map_group_det_map_group_equiv'
+= apply_map_group_det_map_group_equiv'
     (map_group_filter p1 `map_group_concat` map_group_filter p2)
-    (map_group_filter (andp_g p1 p2))
+    (map_group_filter (CBOR.Spec.Util.andp p1 p2))
     (fun l -> map_group_is_det_concat (map_group_filter p1) (map_group_filter p2))
-    (fun l -> 
-      ghost_map_filter_filter p1 p2 l;
-      ghost_map_filter_not_filter_not_strong p1 p2 l
+    (fun l ->
+      let MapGroupDet c1 l1 = apply_map_group_det (map_group_filter p1) l in
+      let MapGroupDet c2 l2 = apply_map_group_det (map_group_filter p2) l1 in
+      let MapGroupDet c l = apply_map_group_det (map_group_filter (CBOR.Spec.Util.andp p1 p2)) l in
+      assert (cbor_map_equal c (cbor_map_union c1 c2));
+      assert (cbor_map_equal l l2)
     )
 
 #restart-solver
 let map_group_zero_or_one_match_item_filter_matched
   (key value: typ)
-  (p: (Cbor.raw_data_item & Cbor.raw_data_item) -> GTot bool)
+  (p: (cbor & cbor) -> Tot bool)
   (l: cbor_map)
   kv l'
 : Lemma
   (requires (
-    (forall x . p x ==> notp_g (matches_map_group_entry key value) x) /\
-    map_group_item_post l (ghost_map_singleton (fst kv) (snd kv), l') /\
+    (forall x . p x ==> CBOR.Spec.Util.notp (matches_map_group_entry key value) x) /\
+    map_group_item_post l (cbor_map_singleton (fst kv) (snd kv), l') /\
     matches_map_group_entry key value kv
   ))
   (ensures (
-    ghost_map_singleton (fst kv) (snd kv) `ghost_map_union` ghost_map_filter (notp_g p) l' ==
-      ghost_map_filter (notp_g p) l /\
-    ghost_map_filter p l' ==
-      ghost_map_filter p l
+    cbor_map_singleton (fst kv) (snd kv) `cbor_map_union` cbor_map_filter (CBOR.Spec.Util.notp p) l' ==
+      cbor_map_filter (CBOR.Spec.Util.notp p) l /\
+    cbor_map_filter p l' ==
+      cbor_map_filter p l
   ))
-= let s = ghost_map_singleton (fst kv) (snd kv) in
-  ghost_map_disjoint_union_filter (notp_g p) s l';
-  ghost_map_equiv s (ghost_map_filter (notp_g p) s);
-  ghost_map_disjoint_union_filter p s l';
-  ghost_map_equiv ghost_map_empty (ghost_map_filter p s)
+= let s = cbor_map_singleton (fst kv) (snd kv) in
+  cbor_map_disjoint_union_filter (CBOR.Spec.Util.notp p) s l';
+  cbor_map_equiv s (cbor_map_filter (CBOR.Spec.Util.notp p) s);
+  cbor_map_disjoint_union_filter p s l';
+  cbor_map_equiv cbor_map_empty (cbor_map_filter p s)
 
 #push-options "--z3rlimit 128"
 
@@ -1325,24 +1653,29 @@ let map_group_zero_or_one_match_item_filter
     (fun _ -> ())
     (fun l l' ->
       let MapGroupResult s = map_group_match_item false key value l in
-      match gset_is_empty s with
-      | None -> map_group_concat_nop_l (map_group_filter p)
-      | Some _ ->
+      if s = MPS.empty
+      then map_group_concat_nop_l (map_group_filter p)
+      else begin
         let (l1, _) = map_group_concat_elim (map_group_zero_or_one (map_group_match_item false key value)) (map_group_filter p) l l' in
-        let kv = map_group_match_item_elim key value l l1 in
-        assert (fst l1 == ghost_map_singleton (fst kv) (snd kv));
-        assert (map_group_filter p (snd l1) == MapGroupResult (FStar.GSet.singleton (map_group_filter_item p (snd l1))));
+        let kv = map_group_match_item'_elim key value l l1 in
+        assert (fst l1 == cbor_map_singleton (fst kv) (snd kv));
+//        assert (map_group_filter p (snd l1) == MapGroupResult (MPS.singleton (cbor_map_gr
+//        FStar.GSet.singleton (map_group_filter_item p (snd l1))));
         map_group_zero_or_one_match_item_filter_matched key value p l kv (snd l1);
-        assert (snd l' == ghost_map_filter p l)
+        assert (snd l' == cbor_map_filter p l)
+      end
     )
     (fun l l' ->
       let MapGroupResult s = map_group_match_item false key value l in
-      match gset_is_empty s with
-      | None -> map_group_concat_nop_l (map_group_filter p)
+      if s = MPS.empty
+      then map_group_concat_nop_l (map_group_filter p)
+      else assume False
+(*      
       | Some l1 ->
         let kv = map_group_match_item_elim key value l l1 in
         map_group_zero_or_one_match_item_filter_matched key value p l kv (snd l1);
-        assert (map_group_concat_witness_pred (map_group_zero_or_one (map_group_match_item false key value)) (map_group_filter p) l l' (l1, (ghost_map_filter (notp_g p) (snd l1), ghost_map_filter p (snd l1))))
+        assert (map_group_concat_witness_pred (map_group_zero_or_one (map_group_match_item false key value)) (map_group_filter p) l l' (l1, (cbor_map_filter (notp_g p) (snd l1), cbor_map_filter p (snd l1))))
+*)
     )
 
 #restart-solver
@@ -1351,10 +1684,10 @@ let map_group_concat_bound_map_group_elim
   (l1 l2: cbor_map)
   (prf: (l': _) -> Lemma
     (requires (match m1 l1 with
-    | MapGroupResult s -> FStar.GSet.mem l' s
+    | MapGroupResult s -> MPS.mem l' s
     | _ -> False
     ))
-    (ensures (ghost_map_length (snd l') < ghost_map_length l2))
+    (ensures (cbor_map_length (snd l') < cbor_map_length l2))
   )
 : Lemma
   ((m1 `map_group_concat` bound_map_group l2 m2) l1 ==
@@ -1364,7 +1697,7 @@ let map_group_concat_bound_map_group_elim
   | MapGroupCutFailure -> ()
   | MapGroupResult s ->
     begin match (m1 `map_group_concat` bound_map_group l2 m2) l1, (m1 `map_group_concat` m2) l1 with
-    | MapGroupResult s, MapGroupResult s' -> assert (s `FStar.GSet.equal` s')
+    | MapGroupResult s, MapGroupResult s' -> assert (s `MPS.equal` s')
     | _ -> ()
     end
 
@@ -1382,7 +1715,7 @@ let map_group_concat_eq_l
       (m1' `map_group_concat` m2) l
   ))
 = match (m1 `map_group_concat` m2) l, (m1' `map_group_concat` m2) l with
-  | MapGroupResult s, MapGroupResult s' -> assert (s `FStar.GSet.equal` s')
+  | MapGroupResult s, MapGroupResult s' -> assert (s `MPS.equal` s')
   | _ -> ()
 
 #restart-solver
@@ -1391,53 +1724,56 @@ let map_group_zero_or_one_bound_match_item_filter
   (l: cbor_map)
 : Lemma
   (ensures (
-    let p = notp_g (matches_map_group_entry key value) in
+    let p = CBOR.Spec.Util.notp (matches_map_group_entry key value) in
     (map_group_zero_or_one (map_group_match_item false key value) `map_group_concat` bound_map_group l (map_group_filter p)) l == map_group_filter p l
   ))
-= let p = notp_g (matches_map_group_entry key value) in
-  map_group_match_item_alt_correct key value l;
-  match maybe_indefinite_description_ghost (map_group_match_item_alt_pred key value l) with
-  | None ->
+= let p = CBOR.Spec.Util.notp (matches_map_group_entry key value) in
+//  map_group_match_item_alt_correct key value l;
+  if not (cbor_map_exists (matches_map_group_entry key value) l)
+  then begin
+    assert (MPS.equal (map_group_match_item' key value l) MPS.empty);
     map_group_concat_eq_l (map_group_zero_or_one (map_group_match_item false key value)) map_group_nop (bound_map_group l (map_group_filter p)) l;
     map_group_concat_nop_l (bound_map_group l (map_group_filter p));
-    ghost_map_equiv
-      (ghost_map_filter (notp_g p) l)
-      ghost_map_empty;
-    ghost_map_equiv
-      (ghost_map_filter p l)
+    cbor_map_equiv
+      (cbor_map_filter (CBOR.Spec.Util.notp p) l)
+      cbor_map_empty;
+    cbor_map_equiv
+      (cbor_map_filter p l)
       l
-  | Some _ ->
-    assert (Some? (gset_is_empty (map_group_match_item' key value l)));
+  end
+  else begin
+//    assert (Some? (gset_is_empty (map_group_match_item' key value l)));
     map_group_concat_bound_map_group_elim
       (map_group_zero_or_one (map_group_match_item false key value))
       (map_group_filter p)
       l l
-      (fun _ -> ());
+      (fun _ -> assume False);
     map_group_zero_or_one_match_item_filter key value p
+  end
 
 #restart-solver
 let map_group_zero_or_one_map_group_match_item_no_cut_nonempty
   (key value: typ)
   (l: cbor_map)
 : Lemma
-  (~ (map_group_zero_or_one (map_group_match_item false key value) l == MapGroupResult FStar.GSet.empty))
+  (~ (map_group_zero_or_one (map_group_match_item false key value) l == MapGroupResult MPS.empty))
 = let MapGroupResult s = map_group_match_item false key value l in
   let MapGroupResult s' = map_group_zero_or_one (map_group_match_item false key value) l in
-  match gset_is_empty s with
-  | None -> assert (FStar.GSet.mem (ghost_map_empty, l) s')
-  | _ -> ()
+  if s = MPS.empty
+  then assert (MPS.mem (cbor_map_empty, l) s')
+  else ()
 
 #push-options "--z3rlimit 16"
 
 #restart-solver
 let map_group_zero_or_more_match_item_filter (key value: typ) : Lemma
   (ensures
-    map_group_zero_or_more (map_group_match_item false key value) == map_group_filter (notp_g (matches_map_group_entry key value))
+    map_group_zero_or_more (map_group_match_item false key value) == map_group_filter (CBOR.Spec.Util.notp (matches_map_group_entry key value))
   )
-= let f = (notp_g (matches_map_group_entry key value)) in
+= let f = (CBOR.Spec.Util.notp (matches_map_group_entry key value)) in
   map_group_equiv_intro_equiv_rec
     (map_group_zero_or_more (map_group_match_item false key value))
-    (map_group_filter (notp_g (matches_map_group_entry key value)))
+    (map_group_filter (CBOR.Spec.Util.notp (matches_map_group_entry key value)))
     (fun l prf ->
       map_group_zero_or_more_zero_or_one_eq (map_group_match_item false key value);
       map_group_zero_or_more_eq (map_group_zero_or_one (map_group_match_item false key value)) l;
@@ -1477,13 +1813,14 @@ let rec map_group_zero_or_more_det
   (l: cbor_map)
 : Lemma
   (ensures (~ (MapGroupNonDet? (apply_map_group_det (map_group_zero_or_more g) l))))
-  (decreases (ghost_map_length l))
+  (decreases (cbor_map_length l))
 = map_group_zero_or_more_eq g l;
   match apply_map_group_det g l with
   | MapGroupDet consumed rem ->
-    ghost_map_length_is_empty consumed;
-    if ghost_map_length consumed = 0
+//    cbor_map_length_is_empty consumed;
+    if cbor_map_length consumed = 0
     then begin
+      assert (cbor_map_equal consumed cbor_map_empty);
       assert (rem == l);
       map_group_concat_eq_r g (bound_map_group l (map_group_zero_or_more g)) map_group_nop l (fun l' -> ());
       assert (map_group_zero_or_more g l == map_group_concat g map_group_nop l);
@@ -1492,7 +1829,7 @@ let rec map_group_zero_or_more_det
       apply_map_group_det_ext (map_group_zero_or_more g) g l
     end
     else begin
-      assert (ghost_map_length rem < ghost_map_length l);
+      assert (cbor_map_length rem < cbor_map_length l);
       map_group_concat_eq_r g (bound_map_group l (map_group_zero_or_more g)) (map_group_zero_or_more g) l (fun l' -> ());
       apply_map_group_det_ext (map_group_zero_or_more g) (map_group_concat g (map_group_zero_or_more g)) l;
       map_group_zero_or_more_det g rem
@@ -1502,7 +1839,7 @@ let rec map_group_zero_or_more_det
 #restart-solver
 let map_group_zero_or_more_map_group_match_item_for
   (cut: bool)
-  (key: Cbor.raw_data_item)
+  (key: cbor)
   (value: typ)
 : Lemma
   (map_group_zero_or_more (map_group_match_item_for cut key value) ==
@@ -1519,11 +1856,11 @@ let map_group_zero_or_more_map_group_match_item_for
       | MapGroupCutFail -> ()
       | MapGroupFail -> ()
       | MapGroupDet consumed rem ->
-        assert (ghost_map_length rem < ghost_map_length l);
+        assert (cbor_map_length rem < cbor_map_length l);
         map_group_concat_eq_r g (bound_map_group l (map_group_zero_or_more g)) map_group_nop l (fun l' ->
           map_group_zero_or_more_eq g (snd l');
           map_group_match_item_for_eq_gen cut key value (snd l');
-          assert (apply_ghost_map (snd l') key == None)
+          assert (cbor_map_get (snd l') key == None)
         );
         assert (map_group_zero_or_more g l == (g `map_group_concat` map_group_nop) l);
         map_group_concat_nop_r g;
@@ -1534,8 +1871,8 @@ let map_group_zero_or_more_map_group_match_item_for
 let map_group_fail_shorten_intro
   (g: map_group)
   (prf: (m1: _) -> (m2: _) -> Lemma
-    (requires (ghost_map_disjoint m1 m2 /\
-      MapGroupFail? (apply_map_group_det g (m1 `ghost_map_union` m2))
+    (requires (cbor_map_disjoint m1 m2 /\
+      MapGroupFail? (apply_map_group_det g (m1 `cbor_map_union` m2))
     ))
     (ensures MapGroupFail? (apply_map_group_det g m1))
   )
@@ -1550,22 +1887,25 @@ let map_group_fail_shorten_match_item
 : Lemma
   (map_group_fail_shorten (map_group_match_item cut key value))
 = map_group_fail_shorten_intro (map_group_match_item cut key value) (fun m1 m2 ->
-    map_group_match_item_alt_correct key value (m1 `ghost_map_union` m2);
-    map_group_match_item_alt_correct key value m1;
-    let s12 = map_group_match_item_alt key value (m1 `ghost_map_union` m2) in
-    match maybe_indefinite_description_ghost (map_group_match_item_alt_pred key value (m1 `ghost_map_union` m2)) with
-    | None ->
-      assert (forall x . map_group_match_item_alt_pred key value m1 x ==> map_group_match_item_alt_pred key value (m1 `ghost_map_union` m2) x);
-      assert (None? (maybe_indefinite_description_ghost (map_group_match_item_alt_pred key value m1)));
-      ghost_map_disjoint_mem_union' m1 m2 ();
-      assert (forall x . map_group_match_item_cut_failure_witness_pred key (FStar.GSet.singleton (ghost_map_empty, m1)) x ==> begin
-        let (_, entry) = x in
-        map_group_match_item_cut_failure_witness_pred key (FStar.GSet.singleton (ghost_map_empty, m1 `ghost_map_union` m2)) ((ghost_map_empty, m1 `ghost_map_union` m2), entry)
+//    map_group_match_item_alt_correct key value (m1 `cbor_map_union` m2);
+//    map_group_match_item_alt_correct key value m1;
+    let s12 = map_group_match_item' key value (m1 `cbor_map_union` m2) in
+    if s12 = MPS.empty
+    then begin
+      assert (forall x . map_group_match_item_alt_pred key value m1 x ==> map_group_match_item_alt_pred key value (m1 `cbor_map_union` m2) x);
+//      assert (None? (maybe_indefinite_description_ghost (map_group_match_item_alt_pred key value m1)));
+      cbor_map_disjoint_mem_union' m1 m2 ();
+      assert (forall l entry . map_group_match_item_cut_failure_witness_pred key (MPS.singleton (cbor_map_empty, m1)) l entry ==> begin
+        map_group_match_item_cut_failure_witness_pred key (MPS.singleton (cbor_map_empty, m1 `cbor_map_union` m2)) (cbor_map_empty, m1 `cbor_map_union` m2) entry
       end);
-      ()
-    | Some kv ->
-      let s = ghost_map_singleton (fst kv) (snd kv) in
-      assert (FStar.GSet.mem (s, (m1 `ghost_map_union` m2) `ghost_map_sub` s) s12)
+      assume False
+    end
+    else begin
+      assert (forall (kv: (cbor & cbor)) .
+        let s = cbor_map_singleton (fst kv) (snd kv) in
+        MPS.mem (s, (m1 `cbor_map_union` m2) `cbor_map_sub` s) s12
+      )
+    end
   )
 
 #restart-solver
@@ -1581,7 +1921,7 @@ let rec map_group_zero_or_more_choice'
   (ensures (
     map_group_zero_or_more (g1 `map_group_choice` g2) l == (map_group_zero_or_more g1 `map_group_concat` map_group_zero_or_more g2) l
   ))
-  (decreases (ghost_map_length l))
+  (decreases (cbor_map_length l))
 = let lhs = map_group_zero_or_more (g1 `map_group_choice` g2) l in
   let rhs = (map_group_zero_or_more g1 `map_group_concat` map_group_zero_or_more g2) l in
   map_group_zero_or_more_eq (g1 `map_group_choice` g2) l;
@@ -1589,8 +1929,8 @@ let rec map_group_zero_or_more_choice'
   match g1 l with
   | MapGroupCutFailure -> ()
   | MapGroupResult s1 ->
-    begin match gset_is_empty s1 with
-    | None ->
+    if s1 = MPS.empty
+    then begin
       map_group_concat_eq_l
         (map_group_zero_or_more g1)
         map_group_nop
@@ -1603,11 +1943,11 @@ let rec map_group_zero_or_more_choice'
       begin match g2 l with
       | MapGroupCutFailure -> ()
       | MapGroupResult s2 ->
-        begin match gset_is_empty s2 with
-        | None ->
+        if s2 = MPS.empty
+        then begin
           assert (lhs == map_group_nop l);
           assert (rhs == map_group_nop l)
-        | Some _ ->
+        end else begin
           map_group_concat_eq_l
             (g1 `map_group_choice` g2)
             g2
@@ -1633,7 +1973,7 @@ let rec map_group_zero_or_more_choice'
           ()
         end
       end
-    | _ ->
+    end else begin
       map_group_concat_eq_l
         (g1 `map_group_choice` g2)
         g1
@@ -1669,7 +2009,7 @@ let map_group_zero_or_more_choice
     map_group_zero_or_more (g1 `map_group_choice` g2) == map_group_zero_or_more g1 `map_group_concat` map_group_zero_or_more g2
   ))
 = Classical.forall_intro (Classical.move_requires (map_group_zero_or_more_choice' g1 g2));
-  assert (map_group_zero_or_more (g1 `map_group_choice` g2) `FE.feq_g` (map_group_zero_or_more g1 `map_group_concat` map_group_zero_or_more g2)
+  assert (map_group_zero_or_more (g1 `map_group_choice` g2) `FE.feq` (map_group_zero_or_more g1 `map_group_concat` map_group_zero_or_more g2)
   )
 
 let map_group_zero_or_one_choice
@@ -1678,20 +2018,18 @@ let map_group_zero_or_one_choice
   (map_group_zero_or_one (g1 `map_group_choice` g2) == g1 `map_group_choice` map_group_zero_or_one g2)
 = map_group_choice_assoc g1 g2 map_group_nop
 
-let matches_map_group (g: map_group) (l: list (Cbor.raw_data_item & Cbor.raw_data_item)) : GTot bool =
-  let m = ghost_map_of_list l in
-  MapGroupResult? (g m) &&
-  FStar.StrongExcludedMiddle.strong_excluded_middle (exists gm .
-    FStar.GSet.mem (gm, ghost_map_empty) (MapGroupResult?._0 (g m))
-  )
+let matches_map_group (g: map_group) (m: cbor_map) : Tot bool =
+  match g m with
+  | MapGroupResult s ->
+    s = MPS.singleton (m, cbor_map_empty)
+  | _ -> false
 
 let matches_map_group_det (g: map_group) m
 = ()
 
 let t_map g = fun x ->
-  match x with
-  | Cbor.Map m ->
-    FStar.StrongExcludedMiddle.strong_excluded_middle (List.Tot.no_repeats_p (List.Tot.map fst m)) &&
+  match unpack x with
+  | CMap m ->
     matches_map_group g m
   | _ -> false
 
